@prefix : <http://www.semanticweb.org/alex/ontologies/2024/4/Flight_Satisfaction_Surveys#> .
@prefix owl: <http://www.w3.org/2002/07/owl#> .
@prefix rdf: <http://www.w3.org/1999/02/22-rdf-syntax-ns#> .
@prefix xml: <http://www.w3.org/XML/1998/namespace> .
@prefix xsd: <http://www.w3.org/2001/XMLSchema#> .
@prefix rdfs: <http://www.w3.org/2000/01/rdf-schema#> .
@base <http://www.semanticweb.org/alex/ontologies/2024/4/Flight_Satisfaction_Surveys#> .

<http://www.semanticweb.org/alex/ontologies/2024/4/Flight_Satisfaction_Surveys> rdf:type owl:Ontology ;
                                                                                 rdfs:comment """@Author:
Alexander Vargas Pierola""" .

#################################################################
#    Annotation properties
#################################################################

###  http://www.w3.org/2000/01/rdf-schema#comment
rdfs:comment rdfs:domain <http://www.semanticweb.org/alex/ontologies/2024/4/Flight_Satisfaction_Surveys/FlightSurvey> .


###  http://www.w3.org/2000/01/rdf-schema#sameAs
rdfs:sameAs rdf:type owl:AnnotationProperty ;
            rdfs:subPropertyOf rdfs:comment .


#################################################################
#    Object Properties
#################################################################

###  http://www.semanticweb.org/alex/ontologies/2024/4/Flight_Satisfaction_Surveys/hasAirline
<http://www.semanticweb.org/alex/ontologies/2024/4/Flight_Satisfaction_Surveys/hasAirline> rdf:type owl:ObjectProperty ;
                                                                                           rdfs:domain <http://www.semanticweb.org/alex/ontologies/2024/4/Flight_Satisfaction_Surveys/FlightSurvey> ;
                                                                                           rdfs:range <http://www.semanticweb.org/alex/ontologies/2024/4/Flight_Satisfaction_Surveys/Airline> ;
                                                                                           rdfs:comment "Relates a flight survey to the airline associated with it." ;
                                                                                           rdfs:label "has Airline" .


###  http://www.semanticweb.org/alex/ontologies/2024/4/Flight_Satisfaction_Surveys/hasComment
<http://www.semanticweb.org/alex/ontologies/2024/4/Flight_Satisfaction_Surveys/hasComment> rdf:type owl:ObjectProperty ;
                                                                                           rdfs:domain <http://www.semanticweb.org/alex/ontologies/2024/4/Flight_Satisfaction_Surveys/FlightSurvey> ;
                                                                                           rdfs:range <http://www.semanticweb.org/alex/ontologies/2024/4/Flight_Satisfaction_Surveys/Passenger> ;
                                                                                           rdfs:label "has Comment" .


###  http://www.semanticweb.org/alex/ontologies/2024/4/Flight_Satisfaction_Surveys/hasFlightDetails
<http://www.semanticweb.org/alex/ontologies/2024/4/Flight_Satisfaction_Surveys/hasFlightDetails> rdf:type owl:ObjectProperty ;
                                                                                                 rdfs:domain <http://www.semanticweb.org/alex/ontologies/2024/4/Flight_Satisfaction_Surveys/FlightSurvey> ;
                                                                                                 rdfs:range <http://www.semanticweb.org/alex/ontologies/2024/4/Flight_Satisfaction_Surveys/FlightDetails> ;
                                                                                                 rdfs:comment "Relates a flight survey to the details of the flight it pertains to." ;
                                                                                                 rdfs:label "has Flight Details" .


###  http://www.semanticweb.org/alex/ontologies/2024/4/Flight_Satisfaction_Surveys/hasFlightDuration
<http://www.semanticweb.org/alex/ontologies/2024/4/Flight_Satisfaction_Surveys/hasFlightDuration> rdf:type owl:ObjectProperty ;
                                                                                                  rdfs:domain <http://www.semanticweb.org/alex/ontologies/2024/4/Flight_Satisfaction_Surveys/Airline> ;
                                                                                                  rdfs:range <http://www.semanticweb.org/alex/ontologies/2024/4/Flight_Satisfaction_Surveys/FlightDetails> ;
                                                                                                  rdfs:label "has Flight Duration" .


###  http://www.semanticweb.org/alex/ontologies/2024/4/Flight_Satisfaction_Surveys/hasFlightFrequency
<http://www.semanticweb.org/alex/ontologies/2024/4/Flight_Satisfaction_Surveys/hasFlightFrequency> rdf:type owl:ObjectProperty ;
                                                                                                   rdfs:domain <http://www.semanticweb.org/alex/ontologies/2024/4/Flight_Satisfaction_Surveys/Airline> ;
                                                                                                   rdfs:range <http://www.semanticweb.org/alex/ontologies/2024/4/Flight_Satisfaction_Surveys/FlightDetails> ;
                                                                                                   rdfs:label "has Flight Frequency" .


###  http://www.semanticweb.org/alex/ontologies/2024/4/Flight_Satisfaction_Surveys/hasPassenger
<http://www.semanticweb.org/alex/ontologies/2024/4/Flight_Satisfaction_Surveys/hasPassenger> rdf:type owl:ObjectProperty ;
                                                                                             rdfs:domain <http://www.semanticweb.org/alex/ontologies/2024/4/Flight_Satisfaction_Surveys/FlightSurvey> ;
                                                                                             rdfs:range <http://www.semanticweb.org/alex/ontologies/2024/4/Flight_Satisfaction_Surveys/Passenger> ;
                                                                                             rdfs:comment "Relates a flight survey to the passenger who participated in it." ;
                                                                                             rdfs:label "has Passenger" .


#################################################################
#    Data properties
#################################################################

###  http://www.semanticweb.org/alex/ontologies/2024/4/Flight_Satisfaction_Surveys/Aircraft
<http://www.semanticweb.org/alex/ontologies/2024/4/Flight_Satisfaction_Surveys/Aircraft> rdf:type owl:DatatypeProperty ;
                                                                                         rdfs:subPropertyOf owl:topDataProperty ;
                                                                                         rdfs:domain <http://www.semanticweb.org/alex/ontologies/2024/4/Flight_Satisfaction_Surveys/FlightDetails> ;
                                                                                         rdfs:range xsd:string ;
                                                                                         rdfs:comment "The type or model of the aircraft used for the flight." ;
                                                                                         rdfs:label "Aircraft" .


###  http://www.semanticweb.org/alex/ontologies/2024/4/Flight_Satisfaction_Surveys/CabinStaffService
<http://www.semanticweb.org/alex/ontologies/2024/4/Flight_Satisfaction_Surveys/CabinStaffService> rdf:type owl:DatatypeProperty ;
                                                                                                  rdfs:subPropertyOf owl:topDataProperty ;
                                                                                                  rdfs:domain <http://www.semanticweb.org/alex/ontologies/2024/4/Flight_Satisfaction_Surveys/FlightSurvey> ;
                                                                                                  rdfs:range xsd:integer ;
                                                                                                  rdfs:comment "The rating or score given by the passenger for the service provided by the cabin staff." ;
                                                                                                  rdfs:label "Cabin Staff Service" .


###  http://www.semanticweb.org/alex/ontologies/2024/4/Flight_Satisfaction_Surveys/Comment
<http://www.semanticweb.org/alex/ontologies/2024/4/Flight_Satisfaction_Surveys/Comment> rdf:type owl:DatatypeProperty ;
                                                                                        rdfs:subPropertyOf owl:topDataProperty ;
                                                                                        rdfs:domain <http://www.semanticweb.org/alex/ontologies/2024/4/Flight_Satisfaction_Surveys/FlightSurvey> ;
                                                                                        rdfs:range xsd:string ;
                                                                                        rdfs:comment "The detailed comment provided by the passenger about their flight experience." ;
                                                                                        rdfs:label "Comment" .


###  http://www.semanticweb.org/alex/ontologies/2024/4/Flight_Satisfaction_Surveys/CommentTitle
<http://www.semanticweb.org/alex/ontologies/2024/4/Flight_Satisfaction_Surveys/CommentTitle> rdf:type owl:DatatypeProperty ;
                                                                                             rdfs:subPropertyOf owl:topDataProperty ;
                                                                                             rdfs:domain <http://www.semanticweb.org/alex/ontologies/2024/4/Flight_Satisfaction_Surveys/FlightSurvey> ;
                                                                                             rdfs:range xsd:string ;
                                                                                             rdfs:comment "The title of the passenger's comment about their flight experience." ;
                                                                                             rdfs:label "Comment Title" .


###  http://www.semanticweb.org/alex/ontologies/2024/4/Flight_Satisfaction_Surveys/DateFlown
<http://www.semanticweb.org/alex/ontologies/2024/4/Flight_Satisfaction_Surveys/DateFlown> rdf:type owl:DatatypeProperty ;
                                                                                          rdfs:subPropertyOf owl:topDataProperty ;
                                                                                          rdfs:domain <http://www.semanticweb.org/alex/ontologies/2024/4/Flight_Satisfaction_Surveys/FlightDetails> ;
                                                                                          rdfs:range xsd:dateTime ;
                                                                                          rdfs:comment "The date when the flight was taken or flown." ;
                                                                                          rdfs:label "Date Flown" .


###  http://www.semanticweb.org/alex/ontologies/2024/4/Flight_Satisfaction_Surveys/DatePublished
<http://www.semanticweb.org/alex/ontologies/2024/4/Flight_Satisfaction_Surveys/DatePublished> rdf:type owl:DatatypeProperty ;
                                                                                              rdfs:subPropertyOf owl:topDataProperty ;
                                                                                              rdfs:domain <http://www.semanticweb.org/alex/ontologies/2024/4/Flight_Satisfaction_Surveys/FlightSurvey> ;
                                                                                              rdfs:range xsd:dateTime ;
                                                                                              rdfs:comment "The date when the flight survey was published or made available." ;
                                                                                              rdfs:label "Date Published" .


###  http://www.semanticweb.org/alex/ontologies/2024/4/Flight_Satisfaction_Surveys/Destination
<http://www.semanticweb.org/alex/ontologies/2024/4/Flight_Satisfaction_Surveys/Destination> rdf:type owl:DatatypeProperty ;
                                                                                            rdfs:subPropertyOf owl:topDataProperty ;
                                                                                            rdfs:domain <http://www.semanticweb.org/alex/ontologies/2024/4/Flight_Satisfaction_Surveys/FlightDetails> ;
                                                                                            rdfs:range xsd:string ;
                                                                                            rdfs:comment "The arrival location or destination of the flight." ;
                                                                                            rdfs:label "Destination" .


###  http://www.semanticweb.org/alex/ontologies/2024/4/Flight_Satisfaction_Surveys/FoodAndBeverages
<http://www.semanticweb.org/alex/ontologies/2024/4/Flight_Satisfaction_Surveys/FoodAndBeverages> rdf:type owl:DatatypeProperty ;
                                                                                                 rdfs:subPropertyOf owl:topDataProperty ;
                                                                                                 rdfs:domain <http://www.semanticweb.org/alex/ontologies/2024/4/Flight_Satisfaction_Surveys/FlightSurvey> ;
                                                                                                 rdfs:range xsd:integer ;
                                                                                                 rdfs:comment "The rating or score given by the passenger for the quality of food and beverages provided during the flight." ;
                                                                                                 rdfs:label "Food And Beverages" .


###  http://www.semanticweb.org/alex/ontologies/2024/4/Flight_Satisfaction_Surveys/GroundService
<http://www.semanticweb.org/alex/ontologies/2024/4/Flight_Satisfaction_Surveys/GroundService> rdf:type owl:DatatypeProperty ;
                                                                                              rdfs:subPropertyOf owl:topDataProperty ;
                                                                                              rdfs:domain <http://www.semanticweb.org/alex/ontologies/2024/4/Flight_Satisfaction_Surveys/FlightSurvey> ;
                                                                                              rdfs:range xsd:integer ;
                                                                                              rdfs:comment "The rating or score given by the passenger for the ground services provided at the airport." ;
                                                                                              rdfs:label "Ground Service" .


###  http://www.semanticweb.org/alex/ontologies/2024/4/Flight_Satisfaction_Surveys/InflightEntertainment
<http://www.semanticweb.org/alex/ontologies/2024/4/Flight_Satisfaction_Surveys/InflightEntertainment> rdf:type owl:DatatypeProperty ;
                                                                                                      rdfs:subPropertyOf owl:topDataProperty ;
                                                                                                      rdfs:domain <http://www.semanticweb.org/alex/ontologies/2024/4/Flight_Satisfaction_Surveys/FlightSurvey> ;
                                                                                                      rdfs:range xsd:integer ;
                                                                                                      rdfs:comment "The rating or score given by the passenger for the quality of inflight entertainment options." ;
                                                                                                      rdfs:label "Inflight Entertainment" .


###  http://www.semanticweb.org/alex/ontologies/2024/4/Flight_Satisfaction_Surveys/Origin
<http://www.semanticweb.org/alex/ontologies/2024/4/Flight_Satisfaction_Surveys/Origin> rdf:type owl:DatatypeProperty ;
                                                                                       rdfs:subPropertyOf owl:topDataProperty ;
                                                                                       rdfs:domain <http://www.semanticweb.org/alex/ontologies/2024/4/Flight_Satisfaction_Surveys/FlightDetails> ;
                                                                                       rdfs:range xsd:string ;
                                                                                       rdfs:comment "The departure location or origin of the flight." ;
                                                                                       rdfs:label "Origin" .


###  http://www.semanticweb.org/alex/ontologies/2024/4/Flight_Satisfaction_Surveys/OverallRating
<http://www.semanticweb.org/alex/ontologies/2024/4/Flight_Satisfaction_Surveys/OverallRating> rdf:type owl:DatatypeProperty ;
                                                                                              rdfs:subPropertyOf owl:topDataProperty ;
                                                                                              rdfs:domain <http://www.semanticweb.org/alex/ontologies/2024/4/Flight_Satisfaction_Surveys/FlightSurvey> ;
                                                                                              rdfs:range [ rdf:type rdfs:Datatype ;
                                                                                                           owl:onDatatype xsd:integer ;
                                                                                                           owl:withRestrictions ( [ xsd:minInclusive 1
                                                                                                                                  ]
                                                                                                                                  [ xsd:maxInclusive 10
                                                                                                                                  ]
                                                                                                                                )
                                                                                                         ] ;
                                                                                              rdfs:comment "The overall rating or score given by the passenger for their flight experience." ;
                                                                                              rdfs:label "Overall Rating" .


###  http://www.semanticweb.org/alex/ontologies/2024/4/Flight_Satisfaction_Surveys/PassengerCountry
<http://www.semanticweb.org/alex/ontologies/2024/4/Flight_Satisfaction_Surveys/PassengerCountry> rdf:type owl:DatatypeProperty ;
                                                                                                 rdfs:subPropertyOf owl:topDataProperty ;
                                                                                                 rdfs:domain <http://www.semanticweb.org/alex/ontologies/2024/4/Flight_Satisfaction_Surveys/Passenger> ;
                                                                                                 rdfs:range xsd:string ;
                                                                                                 rdfs:comment "The country of origin of the passenger." ;
                                                                                                 rdfs:label "Passenger Country" .


###  http://www.semanticweb.org/alex/ontologies/2024/4/Flight_Satisfaction_Surveys/Recommended
<http://www.semanticweb.org/alex/ontologies/2024/4/Flight_Satisfaction_Surveys/Recommended> rdf:type owl:DatatypeProperty ;
                                                                                            rdfs:subPropertyOf owl:topDataProperty ;
                                                                                            rdfs:domain <http://www.semanticweb.org/alex/ontologies/2024/4/Flight_Satisfaction_Surveys/FlightSurvey> ;
                                                                                            rdfs:range [ rdf:type rdfs:Datatype ;
                                                                                                         owl:oneOf [ rdf:type rdf:List ;
                                                                                                                     rdf:first "no" ;
                                                                                                                     rdf:rest [ rdf:type rdf:List ;
                                                                                                                                rdf:first "yes" ;
                                                                                                                                rdf:rest rdf:nil
                                                                                                                              ]
                                                                                                                   ]
                                                                                                       ] ;
                                                                                            rdfs:comment "Indicates whether the passenger would recommend the airline or flight to others" ;
                                                                                            rdfs:label "Recommended" .


###  http://www.semanticweb.org/alex/ontologies/2024/4/Flight_Satisfaction_Surveys/SeatComfort
<http://www.semanticweb.org/alex/ontologies/2024/4/Flight_Satisfaction_Surveys/SeatComfort> rdf:type owl:DatatypeProperty ;
                                                                                            rdfs:subPropertyOf owl:topDataProperty ;
                                                                                            rdfs:domain <http://www.semanticweb.org/alex/ontologies/2024/4/Flight_Satisfaction_Surveys/FlightSurvey> ;
                                                                                            rdfs:range xsd:integer ;
                                                                                            rdfs:comment "The rating or score given by the passenger for the comfort of the seating arrangement." ;
                                                                                            rdfs:label "Seat Comfort" .


###  http://www.semanticweb.org/alex/ontologies/2024/4/Flight_Satisfaction_Surveys/SeatType
<http://www.semanticweb.org/alex/ontologies/2024/4/Flight_Satisfaction_Surveys/SeatType> rdf:type owl:DatatypeProperty ;
                                                                                         rdfs:subPropertyOf owl:topDataProperty ;
                                                                                         rdfs:domain <http://www.semanticweb.org/alex/ontologies/2024/4/Flight_Satisfaction_Surveys/FlightDetails> ;
                                                                                         rdfs:range xsd:string ;
                                                                                         rdfs:comment "The type or class of seating arrangement on the flight, for example economy, business, etc." ;
                                                                                         rdfs:label "Seat Type" .


###  http://www.semanticweb.org/alex/ontologies/2024/4/Flight_Satisfaction_Surveys/TripVerified
<http://www.semanticweb.org/alex/ontologies/2024/4/Flight_Satisfaction_Surveys/TripVerified> rdf:type owl:DatatypeProperty ;
                                                                                             rdfs:subPropertyOf owl:topDataProperty ;
                                                                                             rdfs:domain <http://www.semanticweb.org/alex/ontologies/2024/4/Flight_Satisfaction_Surveys/FlightDetails> ;
                                                                                             rdfs:range xsd:string ;
                                                                                             rdfs:comment "Indicates whether the trip details have been verified by the passenger." ;
                                                                                             rdfs:label "Trip Verified" .


###  http://www.semanticweb.org/alex/ontologies/2024/4/Flight_Satisfaction_Surveys/TypeOfTraveller
<http://www.semanticweb.org/alex/ontologies/2024/4/Flight_Satisfaction_Surveys/TypeOfTraveller> rdf:type owl:DatatypeProperty ;
                                                                                                rdfs:subPropertyOf owl:topDataProperty ;
                                                                                                rdfs:domain <http://www.semanticweb.org/alex/ontologies/2024/4/Flight_Satisfaction_Surveys/Passenger> ;
                                                                                                rdfs:range xsd:string ;
                                                                                                rdfs:comment "The type or category of the passenger, for example business traveler, leisure traveler, etc." ;
                                                                                                rdfs:label "Type Of Traveller" .


###  http://www.semanticweb.org/alex/ontologies/2024/4/Flight_Satisfaction_Surveys/ValueForMoney
<http://www.semanticweb.org/alex/ontologies/2024/4/Flight_Satisfaction_Surveys/ValueForMoney> rdf:type owl:DatatypeProperty ;
                                                                                              rdfs:subPropertyOf owl:topDataProperty ;
                                                                                              rdfs:domain <http://www.semanticweb.org/alex/ontologies/2024/4/Flight_Satisfaction_Surveys/FlightSurvey> ;
                                                                                              rdfs:range xsd:integer ;
                                                                                              rdfs:comment "The rating or score given by the passenger for the perceived value for money of the flight experience." ;
                                                                                              rdfs:label "Value For Money" .


###  http://www.semanticweb.org/alex/ontologies/2024/4/Flight_Satisfaction_Surveys/WifiAndConnectivity
<http://www.semanticweb.org/alex/ontologies/2024/4/Flight_Satisfaction_Surveys/WifiAndConnectivity> rdf:type owl:DatatypeProperty ;
                                                                                                    rdfs:subPropertyOf owl:topDataProperty ;
                                                                                                    rdfs:domain <http://www.semanticweb.org/alex/ontologies/2024/4/Flight_Satisfaction_Surveys/FlightSurvey> ;
                                                                                                    rdfs:range xsd:integer ;
                                                                                                    rdfs:label "The rating or score given by the passenger for the quality of Wi-Fi and connectivity services were available during the flight." ,
                                                                                                               "Wifi And Connectivity" .


#################################################################
#    Classes
#################################################################

###  http://www.semanticweb.org/alex/ontologies/2024/4/Flight_Satisfaction_Surveys/Airline
<http://www.semanticweb.org/alex/ontologies/2024/4/Flight_Satisfaction_Surveys/Airline> rdf:type owl:Class ;
                                                                                        rdfs:comment "Represents an airline company providing flight services to passengers." ;
                                                                                        rdfs:label "Airline" .


###  http://www.semanticweb.org/alex/ontologies/2024/4/Flight_Satisfaction_Surveys/ArrivalExperienceSurvey
<http://www.semanticweb.org/alex/ontologies/2024/4/Flight_Satisfaction_Surveys/ArrivalExperienceSurvey> rdf:type owl:Class ;
                                                                                                        rdfs:subClassOf <http://www.semanticweb.org/alex/ontologies/2024/4/Flight_Satisfaction_Surveys/PostFlightSurvey> ;
                                                                                                        rdfs:comment "Represents a survey used to gather feedback from passengers about their experience upon arrival at the destination airport, including customs, immigration, and ground transportation." ;
                                                                                                        rdfs:label "Arrival Experience Survey" .


###  http://www.semanticweb.org/alex/ontologies/2024/4/Flight_Satisfaction_Surveys/BaggageClaimSurvey
<http://www.semanticweb.org/alex/ontologies/2024/4/Flight_Satisfaction_Surveys/BaggageClaimSurvey> rdf:type owl:Class ;
                                                                                                   rdfs:subClassOf <http://www.semanticweb.org/alex/ontologies/2024/4/Flight_Satisfaction_Surveys/PostFlightSurvey> ;
                                                                                                   rdfs:comment "Represents a survey used to gather feedback from passengers about their experience at the baggage claim area, including the efficiency and convenience of baggage retrieval." ;
                                                                                                   rdfs:label "Baggage Claim Survey" .


###  http://www.semanticweb.org/alex/ontologies/2024/4/Flight_Satisfaction_Surveys/BasicEconomyClassPassenger
<http://www.semanticweb.org/alex/ontologies/2024/4/Flight_Satisfaction_Surveys/BasicEconomyClassPassenger> rdf:type owl:Class ;
                                                                                                           rdfs:subClassOf <http://www.semanticweb.org/alex/ontologies/2024/4/Flight_Satisfaction_Surveys/EconomyClassPassenger> ;
                                                                                                           rdfs:comment "Represents a passenger traveling in the basic or standard economy class cabin of an aircraft, offering essential amenities and services at a lower cost." ;
                                                                                                           rdfs:label "Basic Economy Class Passenger" .


###  http://www.semanticweb.org/alex/ontologies/2024/4/Flight_Satisfaction_Surveys/BusinessClassPassenger
<http://www.semanticweb.org/alex/ontologies/2024/4/Flight_Satisfaction_Surveys/BusinessClassPassenger> rdf:type owl:Class ;
                                                                                                       rdfs:subClassOf <http://www.semanticweb.org/alex/ontologies/2024/4/Flight_Satisfaction_Surveys/Passenger> ;
                                                                                                       rdfs:comment "Represents a passenger who travels in the business class cabin of an aircraft, normally offering enhanced amenities and services compared to economy class." ;
                                                                                                       rdfs:label "Business Class Passenger" ;
                                                                                                       rdfs:sameAs "http://dbpedia.org/resource/Business_class" .


###  http://www.semanticweb.org/alex/ontologies/2024/4/Flight_Satisfaction_Surveys/CrewSatisfactionSurvey
<http://www.semanticweb.org/alex/ontologies/2024/4/Flight_Satisfaction_Surveys/CrewSatisfactionSurvey> rdf:type owl:Class ;
                                                                                                       rdfs:subClassOf <http://www.semanticweb.org/alex/ontologies/2024/4/Flight_Satisfaction_Surveys/EmployeeSurvey> ;
                                                                                                       rdfs:comment "Represents a survey conducted to gather feedback from airline crew members about their job satisfaction, working conditions, and overall experience in their roles." ;
                                                                                                       rdfs:label "Crew Satisfaction Survey" .


###  http://www.semanticweb.org/alex/ontologies/2024/4/Flight_Satisfaction_Surveys/CustomerSurvey
<http://www.semanticweb.org/alex/ontologies/2024/4/Flight_Satisfaction_Surveys/CustomerSurvey> rdf:type owl:Class ;
                                                                                               rdfs:subClassOf <http://www.semanticweb.org/alex/ontologies/2024/4/Flight_Satisfaction_Surveys/FlightSurvey> ;
                                                                                               rdfs:comment "Represents a survey used to gather feedback from customers about their experience with a product or service." ;
                                                                                               rdfs:label "Customer Survey" .


###  http://www.semanticweb.org/alex/ontologies/2024/4/Flight_Satisfaction_Surveys/DomesticFlight
<http://www.semanticweb.org/alex/ontologies/2024/4/Flight_Satisfaction_Surveys/DomesticFlight> rdf:type owl:Class ;
                                                                                               rdfs:subClassOf <http://www.semanticweb.org/alex/ontologies/2024/4/Flight_Satisfaction_Surveys/Airline> ;
                                                                                               rdfs:comment "Represents a flight that operates within the borders of a single country, without crossing international boundaries." ;
                                                                                               rdfs:label "Domestic Flight" .


###  http://www.semanticweb.org/alex/ontologies/2024/4/Flight_Satisfaction_Surveys/DomesticLongHaulFlight
<http://www.semanticweb.org/alex/ontologies/2024/4/Flight_Satisfaction_Surveys/DomesticLongHaulFlight> rdf:type owl:Class ;
                                                                                                       rdfs:subClassOf <http://www.semanticweb.org/alex/ontologies/2024/4/Flight_Satisfaction_Surveys/LongHaulFlight> ;
                                                                                                       rdfs:comment "Represents a long-haul flight operating within a country or region, covering extensive distances." ;
                                                                                                       rdfs:label "Domestic Long Haul Flight" .


###  http://www.semanticweb.org/alex/ontologies/2024/4/Flight_Satisfaction_Surveys/DomesticRegionalAirline
<http://www.semanticweb.org/alex/ontologies/2024/4/Flight_Satisfaction_Surveys/DomesticRegionalAirline> rdf:type owl:Class ;
                                                                                                        rdfs:subClassOf <http://www.semanticweb.org/alex/ontologies/2024/4/Flight_Satisfaction_Surveys/RegionalAirline> ;
                                                                                                        rdfs:comment "Represents a regional airline specializing in offering flight services within a specific country or region." ;
                                                                                                        rdfs:label "Domestic Regional Airline" .


###  http://www.semanticweb.org/alex/ontologies/2024/4/Flight_Satisfaction_Surveys/EconomyClassPassenger
<http://www.semanticweb.org/alex/ontologies/2024/4/Flight_Satisfaction_Surveys/EconomyClassPassenger> rdf:type owl:Class ;
                                                                                                      rdfs:subClassOf <http://www.semanticweb.org/alex/ontologies/2024/4/Flight_Satisfaction_Surveys/Passenger> ;
                                                                                                      rdfs:comment "Represents a passenger who travels in the economy class cabin of an aircraft, normally offering standard amenities and services." ;
                                                                                                      rdfs:label "Economy Class Passenger" .


###  http://www.semanticweb.org/alex/ontologies/2024/4/Flight_Satisfaction_Surveys/EliteFrequentFlyer
<http://www.semanticweb.org/alex/ontologies/2024/4/Flight_Satisfaction_Surveys/EliteFrequentFlyer> rdf:type owl:Class ;
                                                                                                   rdfs:subClassOf <http://www.semanticweb.org/alex/ontologies/2024/4/Flight_Satisfaction_Surveys/FrequentFlyer> ;
                                                                                                   rdfs:comment "Represents a frequent flyer with elite status in an airline's loyalty program, enjoying exclusive benefits, privileges, and rewards." ;
                                                                                                   rdfs:label "Elite Frequent Flyer" .


###  http://www.semanticweb.org/alex/ontologies/2024/4/Flight_Satisfaction_Surveys/EmployeeSurvey
<http://www.semanticweb.org/alex/ontologies/2024/4/Flight_Satisfaction_Surveys/EmployeeSurvey> rdf:type owl:Class ;
                                                                                               rdfs:subClassOf <http://www.semanticweb.org/alex/ontologies/2024/4/Flight_Satisfaction_Surveys/FlightSurvey> ;
                                                                                               rdfs:comment "Represents a survey used to gather feedback from employees about their job satisfaction, work environment, and other related aspects." ;
                                                                                               rdfs:label "Employee Survey" .


###  http://www.semanticweb.org/alex/ontologies/2024/4/Flight_Satisfaction_Surveys/ExperienceSurvey
<http://www.semanticweb.org/alex/ontologies/2024/4/Flight_Satisfaction_Surveys/ExperienceSurvey> rdf:type owl:Class ;
                                                                                                 rdfs:subClassOf <http://www.semanticweb.org/alex/ontologies/2024/4/Flight_Satisfaction_Surveys/CustomerSurvey> ;
                                                                                                 rdfs:comment "Represents a survey designed to gather feedback from customers about their overall experience, including interactions, perceptions, and sentiments." ;
                                                                                                 rdfs:label "Experience Survey" .


###  http://www.semanticweb.org/alex/ontologies/2024/4/Flight_Satisfaction_Surveys/FamilyLeisureTraveler
<http://www.semanticweb.org/alex/ontologies/2024/4/Flight_Satisfaction_Surveys/FamilyLeisureTraveler> rdf:type owl:Class ;
                                                                                                      rdfs:subClassOf <http://www.semanticweb.org/alex/ontologies/2024/4/Flight_Satisfaction_Surveys/LeisureTraveler> ;
                                                                                                      rdfs:comment "Represents a leisure traveler who travels with family members for vacation, holidays, or recreational activities, often seeking family-friendly travel options." ;
                                                                                                      rdfs:label "Family Leisure Traveler" .


###  http://www.semanticweb.org/alex/ontologies/2024/4/Flight_Satisfaction_Surveys/FlightDetails
<http://www.semanticweb.org/alex/ontologies/2024/4/Flight_Satisfaction_Surveys/FlightDetails> rdf:type owl:Class ;
                                                                                              rdfs:comment "Represents the specific details of a flight, including its route, duration, and the main information." ;
                                                                                              rdfs:label "Flight Details" .


###  http://www.semanticweb.org/alex/ontologies/2024/4/Flight_Satisfaction_Surveys/FlightSurvey
<http://www.semanticweb.org/alex/ontologies/2024/4/Flight_Satisfaction_Surveys/FlightSurvey> rdf:type owl:Class ;
                                                                                             rdfs:subClassOf [ rdf:type owl:Restriction ;
                                                                                                               owl:onProperty <http://www.semanticweb.org/alex/ontologies/2024/4/Flight_Satisfaction_Surveys/hasAirline> ;
                                                                                                               owl:qualifiedCardinality "1"^^xsd:nonNegativeInteger ;
                                                                                                               owl:onClass <http://www.semanticweb.org/alex/ontologies/2024/4/Flight_Satisfaction_Surveys/FlightSurvey>
                                                                                                             ] ,
                                                                                                             [ rdf:type owl:Restriction ;
                                                                                                               owl:onProperty <http://www.semanticweb.org/alex/ontologies/2024/4/Flight_Satisfaction_Surveys/hasPassenger> ;
                                                                                                               owl:qualifiedCardinality "1"^^xsd:nonNegativeInteger ;
                                                                                                               owl:onClass <http://www.semanticweb.org/alex/ontologies/2024/4/Flight_Satisfaction_Surveys/FlightSurvey>
                                                                                                             ] ,
                                                                                                             [ rdf:type owl:Restriction ;
                                                                                                               owl:onProperty <http://www.semanticweb.org/alex/ontologies/2024/4/Flight_Satisfaction_Surveys/hasFlightDetails> ;
                                                                                                               owl:maxQualifiedCardinality "1"^^xsd:nonNegativeInteger ;
                                                                                                               owl:onClass <http://www.semanticweb.org/alex/ontologies/2024/4/Flight_Satisfaction_Surveys/FlightSurvey>
                                                                                                             ] ;
                                                                                             rdfs:comment "Represents a survey used to gather feedback from different people about their flight experience." ;
                                                                                             rdfs:label "Flight Survey" .


###  http://www.semanticweb.org/alex/ontologies/2024/4/Flight_Satisfaction_Surveys/FrequentFlyer
<http://www.semanticweb.org/alex/ontologies/2024/4/Flight_Satisfaction_Surveys/FrequentFlyer> rdf:type owl:Class ;
                                                                                              rdfs:subClassOf <http://www.semanticweb.org/alex/ontologies/2024/4/Flight_Satisfaction_Surveys/Passenger> ;
                                                                                              rdfs:comment "Represents a passenger who frequently travels by air and may be enrolled in a loyalty program offered by an airline." ;
                                                                                              rdfs:label "Frequent Flyer" .


###  http://www.semanticweb.org/alex/ontologies/2024/4/Flight_Satisfaction_Surveys/FullServiceInternationalAirline
<http://www.semanticweb.org/alex/ontologies/2024/4/Flight_Satisfaction_Surveys/FullServiceInternationalAirline> rdf:type owl:Class ;
                                                                                                                rdfs:subClassOf <http://www.semanticweb.org/alex/ontologies/2024/4/Flight_Satisfaction_Surveys/InternationalAirline> ;
                                                                                                                rdfs:comment "Represents an international airline company that offers comprehensive flight services, including various cabin classes, amenities, and customer services." ;
                                                                                                                rdfs:label "Full Service International Airline" .


###  http://www.semanticweb.org/alex/ontologies/2024/4/Flight_Satisfaction_Surveys/GroundStaffSurvey
<http://www.semanticweb.org/alex/ontologies/2024/4/Flight_Satisfaction_Surveys/GroundStaffSurvey> rdf:type owl:Class ;
                                                                                                  rdfs:subClassOf <http://www.semanticweb.org/alex/ontologies/2024/4/Flight_Satisfaction_Surveys/EmployeeSurvey> ;
                                                                                                  rdfs:comment "Ground Staff Survey" ,
                                                                                                               "Represents a survey used to gather feedback from ground staff employees, such as airport personnel and support staff, about their job satisfaction and work environment." .


###  http://www.semanticweb.org/alex/ontologies/2024/4/Flight_Satisfaction_Surveys/HybridInternationalAirline
<http://www.semanticweb.org/alex/ontologies/2024/4/Flight_Satisfaction_Surveys/HybridInternationalAirline> rdf:type owl:Class ;
                                                                                                           rdfs:subClassOf <http://www.semanticweb.org/alex/ontologies/2024/4/Flight_Satisfaction_Surveys/InternationalAirline> ;
                                                                                                           rdfs:comment "Represents an international airline company that combines elements of both full-service and low-cost carriers, providing a mix of amenities and services." ;
                                                                                                           rdfs:label "Hybrid International Airline" .


###  http://www.semanticweb.org/alex/ontologies/2024/4/Flight_Satisfaction_Surveys/ImmigrationProcessSurvey
<http://www.semanticweb.org/alex/ontologies/2024/4/Flight_Satisfaction_Surveys/ImmigrationProcessSurvey> rdf:type owl:Class ;
                                                                                                         rdfs:subClassOf <http://www.semanticweb.org/alex/ontologies/2024/4/Flight_Satisfaction_Surveys/PostFlightSurvey> ;
                                                                                                         rdfs:comment "Represents a survey used to gather feedback from passengers about their experience with immigration procedures and processes upon arrival at an international destination." ;
                                                                                                         rdfs:label "Immigration Process Survey" .


###  http://www.semanticweb.org/alex/ontologies/2024/4/Flight_Satisfaction_Surveys/InternationalAirline
<http://www.semanticweb.org/alex/ontologies/2024/4/Flight_Satisfaction_Surveys/InternationalAirline> rdf:type owl:Class ;
                                                                                                     rdfs:subClassOf <http://www.semanticweb.org/alex/ontologies/2024/4/Flight_Satisfaction_Surveys/FlightDetails> ;
                                                                                                     rdfs:comment "Represents an airline company that operates flights primarily between different countries or regions." ;
                                                                                                     rdfs:label "International Airline" .


###  http://www.semanticweb.org/alex/ontologies/2024/4/Flight_Satisfaction_Surveys/InternationalFlight
<http://www.semanticweb.org/alex/ontologies/2024/4/Flight_Satisfaction_Surveys/InternationalFlight> rdf:type owl:Class ;
                                                                                                    rdfs:subClassOf <http://www.semanticweb.org/alex/ontologies/2024/4/Flight_Satisfaction_Surveys/Airline> ;
                                                                                                    rdfs:comment "Represents a flight that operates between different countries or across international boundaries." ;
                                                                                                    rdfs:label "International Flight" ;
                                                                                                    rdfs:sameAs "http://dbpedia.org/resource/International_flight" .


###  http://www.semanticweb.org/alex/ontologies/2024/4/Flight_Satisfaction_Surveys/InternationalLongHaulFlight
<http://www.semanticweb.org/alex/ontologies/2024/4/Flight_Satisfaction_Surveys/InternationalLongHaulFlight> rdf:type owl:Class ;
                                                                                                            rdfs:subClassOf <http://www.semanticweb.org/alex/ontologies/2024/4/Flight_Satisfaction_Surveys/LongHaulFlight> ;
                                                                                                            rdfs:comment "Represents a long-haul flight operating between countries or regions, covering extensive distances." ;
                                                                                                            rdfs:label "International Long Haul Flight" .


###  http://www.semanticweb.org/alex/ontologies/2024/4/Flight_Satisfaction_Surveys/InternationalRegionalAirline
<http://www.semanticweb.org/alex/ontologies/2024/4/Flight_Satisfaction_Surveys/InternationalRegionalAirline> rdf:type owl:Class ;
                                                                                                             rdfs:subClassOf <http://www.semanticweb.org/alex/ontologies/2024/4/Flight_Satisfaction_Surveys/RegionalAirline> ;
                                                                                                             rdfs:comment "Represents a regional airline providing flight services to international destinations within a specific geographical region." ;
                                                                                                             rdfs:label "International Regional Airline" .


###  http://www.semanticweb.org/alex/ontologies/2024/4/Flight_Satisfaction_Surveys/LeisureTraveler
<http://www.semanticweb.org/alex/ontologies/2024/4/Flight_Satisfaction_Surveys/LeisureTraveler> rdf:type owl:Class ;
                                                                                                rdfs:subClassOf <http://www.semanticweb.org/alex/ontologies/2024/4/Flight_Satisfaction_Surveys/Passenger> ;
                                                                                                rdfs:comment "Represents a passenger who travels for leisure purposes, such as vacations, holidays, or recreational activities." ;
                                                                                                rdfs:label "Leisure Traveler" .


###  http://www.semanticweb.org/alex/ontologies/2024/4/Flight_Satisfaction_Surveys/LongDomesticFlight
<http://www.semanticweb.org/alex/ontologies/2024/4/Flight_Satisfaction_Surveys/LongDomesticFlight> rdf:type owl:Class ;
                                                                                                   rdfs:subClassOf <http://www.semanticweb.org/alex/ontologies/2024/4/Flight_Satisfaction_Surveys/DomesticFlight> ;
                                                                                                   rdfs:comment "Represents a domestic flight with a relatively long duration, normally covering extensive distances within a country or region." ;
                                                                                                   rdfs:label "Long Domestic Flight" .


###  http://www.semanticweb.org/alex/ontologies/2024/4/Flight_Satisfaction_Surveys/LongHaulFlight
<http://www.semanticweb.org/alex/ontologies/2024/4/Flight_Satisfaction_Surveys/LongHaulFlight> rdf:type owl:Class ;
                                                                                               rdfs:subClassOf <http://www.semanticweb.org/alex/ontologies/2024/4/Flight_Satisfaction_Surveys/Airline> ;
                                                                                               rdfs:comment "Represents a flight with a relatively long duration, normally more than seven hours and covering extensive distances, often between continents." ;
                                                                                               rdfs:label "Long Haul Flight" .


###  http://www.semanticweb.org/alex/ontologies/2024/4/Flight_Satisfaction_Surveys/LongInternationalFlight
<http://www.semanticweb.org/alex/ontologies/2024/4/Flight_Satisfaction_Surveys/LongInternationalFlight> rdf:type owl:Class ;
                                                                                                        rdfs:subClassOf <http://www.semanticweb.org/alex/ontologies/2024/4/Flight_Satisfaction_Surveys/InternationalFlight> ;
                                                                                                        rdfs:comment "Represents an international flight with a relatively long duration, normally covering extensive distances between countries or regions." ;
                                                                                                        rdfs:label "Long International Flight" .


###  http://www.semanticweb.org/alex/ontologies/2024/4/Flight_Satisfaction_Surveys/LowCostCarrier
<http://www.semanticweb.org/alex/ontologies/2024/4/Flight_Satisfaction_Surveys/LowCostCarrier> rdf:type owl:Class ;
                                                                                               rdfs:subClassOf <http://www.semanticweb.org/alex/ontologies/2024/4/Flight_Satisfaction_Surveys/FlightDetails> ;
                                                                                               rdfs:comment "Represents an airline company that offers low-cost flight services, normally with fewer amenities and services compared to traditional airlines." ;
                                                                                               rdfs:label "Low Cost Carrier" ;
                                                                                               rdfs:sameAs "http://dbpedia.org/resource/Low-cost_carrier" .


###  http://www.semanticweb.org/alex/ontologies/2024/4/Flight_Satisfaction_Surveys/LoyaltySurvey
<http://www.semanticweb.org/alex/ontologies/2024/4/Flight_Satisfaction_Surveys/LoyaltySurvey> rdf:type owl:Class ;
                                                                                              rdfs:subClassOf <http://www.semanticweb.org/alex/ontologies/2024/4/Flight_Satisfaction_Surveys/CustomerSurvey> ;
                                                                                              rdfs:comment "Represents a survey aimed at assessing the loyalty, retention, and engagement of customers towards a brand, company, or organization." ;
                                                                                              rdfs:label "Loyalty Survey" .


###  http://www.semanticweb.org/alex/ontologies/2024/4/Flight_Satisfaction_Surveys/MaintenanceStaffSurvey
<http://www.semanticweb.org/alex/ontologies/2024/4/Flight_Satisfaction_Surveys/MaintenanceStaffSurvey> rdf:type owl:Class ;
                                                                                                       rdfs:subClassOf <http://www.semanticweb.org/alex/ontologies/2024/4/Flight_Satisfaction_Surveys/EmployeeSurvey> ;
                                                                                                       rdfs:comment "Represents a survey used to gather feedback from maintenance staff employees, such as aircraft technicians and engineers, about their job satisfaction and work conditions." ;
                                                                                                       rdfs:label "Maintenance Staff Survey" .


###  http://www.semanticweb.org/alex/ontologies/2024/4/Flight_Satisfaction_Surveys/Passenger
<http://www.semanticweb.org/alex/ontologies/2024/4/Flight_Satisfaction_Surveys/Passenger> rdf:type owl:Class ;
                                                                                          rdfs:comment "It represents a traveler taking a flight operated by an airline." ;
                                                                                          rdfs:label "Passenger" .


###  http://www.semanticweb.org/alex/ontologies/2024/4/Flight_Satisfaction_Surveys/PlusEconomyClassPassenger
<http://www.semanticweb.org/alex/ontologies/2024/4/Flight_Satisfaction_Surveys/PlusEconomyClassPassenger> rdf:type owl:Class ;
                                                                                                          rdfs:subClassOf <http://www.semanticweb.org/alex/ontologies/2024/4/Flight_Satisfaction_Surveys/EconomyClassPassenger> ;
                                                                                                          rdfs:comment "Represents a passenger traveling in the plus or upgraded economy class cabin of an aircraft, offering additional amenities and services compared to standard economy class." ;
                                                                                                          rdfs:label "Plus Economy Class Passenger" .


###  http://www.semanticweb.org/alex/ontologies/2024/4/Flight_Satisfaction_Surveys/PostFlightSurvey
<http://www.semanticweb.org/alex/ontologies/2024/4/Flight_Satisfaction_Surveys/PostFlightSurvey> rdf:type owl:Class ;
                                                                                                 rdfs:subClassOf <http://www.semanticweb.org/alex/ontologies/2024/4/Flight_Satisfaction_Surveys/FlightSurvey> ;
                                                                                                 rdfs:comment "Represents a more specific survey used to gather feedback from passengers about their experience after completing a flight, including arrival procedures and baggage claim." ;
                                                                                                 rdfs:label "Post Flight Survey" .


###  http://www.semanticweb.org/alex/ontologies/2024/4/Flight_Satisfaction_Surveys/PremiumBusinessClassPassenger
<http://www.semanticweb.org/alex/ontologies/2024/4/Flight_Satisfaction_Surveys/PremiumBusinessClassPassenger> rdf:type owl:Class ;
                                                                                                              rdfs:subClassOf <http://www.semanticweb.org/alex/ontologies/2024/4/Flight_Satisfaction_Surveys/BusinessClassPassenger> ;
                                                                                                              rdfs:comment "Represents a passenger traveling in the premium or upgraded business class cabin of an aircraft, offering enhanced amenities, services, and comfort." ;
                                                                                                              rdfs:label "Premium Business Class Passenger" .


###  http://www.semanticweb.org/alex/ontologies/2024/4/Flight_Satisfaction_Surveys/RegionalAirline
<http://www.semanticweb.org/alex/ontologies/2024/4/Flight_Satisfaction_Surveys/RegionalAirline> rdf:type owl:Class ;
                                                                                                rdfs:subClassOf <http://www.semanticweb.org/alex/ontologies/2024/4/Flight_Satisfaction_Surveys/FlightDetails> ;
                                                                                                rdfs:comment "Represents an airline company that operates flights within a specific geographical region, often connecting smaller cities and towns." ;
                                                                                                rdfs:label "Regional Airline" .


###  http://www.semanticweb.org/alex/ontologies/2024/4/Flight_Satisfaction_Surveys/RegionalLowCostCarrier
<http://www.semanticweb.org/alex/ontologies/2024/4/Flight_Satisfaction_Surveys/RegionalLowCostCarrier> rdf:type owl:Class ;
                                                                                                       rdfs:subClassOf <http://www.semanticweb.org/alex/ontologies/2024/4/Flight_Satisfaction_Surveys/LowCostCarrier> ;
                                                                                                       rdfs:comment "Represents a low-cost carrier focusing on providing affordable flight services within a specific region or country." ;
                                                                                                       rdfs:label "Regional Low Cost Carrier" .


###  http://www.semanticweb.org/alex/ontologies/2024/4/Flight_Satisfaction_Surveys/SatisfactionSurvey
<http://www.semanticweb.org/alex/ontologies/2024/4/Flight_Satisfaction_Surveys/SatisfactionSurvey> rdf:type owl:Class ;
                                                                                                   rdfs:subClassOf <http://www.semanticweb.org/alex/ontologies/2024/4/Flight_Satisfaction_Surveys/CustomerSurvey> ;
                                                                                                   rdfs:comment "Represents a survey focused on measuring the level of satisfaction or contentment of customers about the flight service." ;
                                                                                                   rdfs:label "Satisfaction Survey" .


###  http://www.semanticweb.org/alex/ontologies/2024/4/Flight_Satisfaction_Surveys/ShortDomesticFlight
<http://www.semanticweb.org/alex/ontologies/2024/4/Flight_Satisfaction_Surveys/ShortDomesticFlight> rdf:type owl:Class ;
                                                                                                    rdfs:subClassOf <http://www.semanticweb.org/alex/ontologies/2024/4/Flight_Satisfaction_Surveys/DomesticFlight> ;
                                                                                                    rdfs:comment "Represents a domestic flight with a relatively short duration, normally covering distances within a certain range." ;
                                                                                                    rdfs:label "Short Domestic Flight" .


###  http://www.semanticweb.org/alex/ontologies/2024/4/Flight_Satisfaction_Surveys/ShortInternationalFlight
<http://www.semanticweb.org/alex/ontologies/2024/4/Flight_Satisfaction_Surveys/ShortInternationalFlight> rdf:type owl:Class ;
                                                                                                         rdfs:subClassOf <http://www.semanticweb.org/alex/ontologies/2024/4/Flight_Satisfaction_Surveys/InternationalFlight> ;
                                                                                                         rdfs:comment "Represents an international flight with a relatively short duration, normally covering distances within a certain range between countries or regions." ;
                                                                                                         rdfs:label "Short International Flight" .


###  http://www.semanticweb.org/alex/ontologies/2024/4/Flight_Satisfaction_Surveys/SoloLeisureTraveler
<http://www.semanticweb.org/alex/ontologies/2024/4/Flight_Satisfaction_Surveys/SoloLeisureTraveler> rdf:type owl:Class ;
                                                                                                    rdfs:subClassOf <http://www.semanticweb.org/alex/ontologies/2024/4/Flight_Satisfaction_Surveys/LeisureTraveler> ;
                                                                                                    rdfs:comment "Represents a leisure traveler who travels alone for personal enjoyment, relaxation, or exploration, seeking travel experiences tailored to individual preferences." ;
                                                                                                    rdfs:label "Solo Leisure Traveler" .


###  http://www.semanticweb.org/alex/ontologies/2024/4/Flight_Satisfaction_Surveys/StandardBusinessClassPassenger
<http://www.semanticweb.org/alex/ontologies/2024/4/Flight_Satisfaction_Surveys/StandardBusinessClassPassenger> rdf:type owl:Class ;
                                                                                                               rdfs:subClassOf <http://www.semanticweb.org/alex/ontologies/2024/4/Flight_Satisfaction_Surveys/BusinessClassPassenger> ;
                                                                                                               rdfs:comment "Represents a passenger traveling in the standard business class cabin of an aircraft, offering typical amenities and services for business-class passengers." ;
                                                                                                               rdfs:label "Standard Business Class Passenger" .


###  http://www.semanticweb.org/alex/ontologies/2024/4/Flight_Satisfaction_Surveys/StandardFrequentFlyer
<http://www.semanticweb.org/alex/ontologies/2024/4/Flight_Satisfaction_Surveys/StandardFrequentFlyer> rdf:type owl:Class ;
                                                                                                      rdfs:subClassOf <http://www.semanticweb.org/alex/ontologies/2024/4/Flight_Satisfaction_Surveys/FrequentFlyer> ;
                                                                                                      rdfs:comment "Represents a frequent flyer enrolled in an airline's loyalty program, earning rewards and benefits based on their travel activity." ;
                                                                                                      rdfs:label "Standard Frequent Flyer" .


###  http://www.semanticweb.org/alex/ontologies/2024/4/Flight_Satisfaction_Surveys/UltraLowCostCarrier
<http://www.semanticweb.org/alex/ontologies/2024/4/Flight_Satisfaction_Surveys/UltraLowCostCarrier> rdf:type owl:Class ;
                                                                                                    rdfs:subClassOf <http://www.semanticweb.org/alex/ontologies/2024/4/Flight_Satisfaction_Surveys/LowCostCarrier> ;
                                                                                                    rdfs:comment "Represents an airline company offering extremely budget-friendly flight services with minimal amenities and additional charges." ;
                                                                                                    rdfs:label "Ultra Low Cost Carrier" .


#################################################################
#    Individuals
#################################################################

###  http://www.semanticweb.org/alex/ontologies/2024/4/Flight_Satisfaction_Surveys/BusinessClassPassengerInstance
<http://www.semanticweb.org/alex/ontologies/2024/4/Flight_Satisfaction_Surveys/BusinessClassPassengerInstance> rdf:type owl:NamedIndividual ,
                                                                                                                        <http://www.semanticweb.org/alex/ontologies/2024/4/Flight_Satisfaction_Surveys/BusinessClassPassenger> ;
                                                                                                               rdfs:comment "Instance for 'Business Class Passenger'" ;
                                                                                                               rdfs:label "Business Class Passenger Instance" .


###  http://www.semanticweb.org/alex/ontologies/2024/4/Flight_Satisfaction_Surveys/CustomerSurveyIntance
<http://www.semanticweb.org/alex/ontologies/2024/4/Flight_Satisfaction_Surveys/CustomerSurveyIntance> rdf:type owl:NamedIndividual ,
                                                                                                               <http://www.semanticweb.org/alex/ontologies/2024/4/Flight_Satisfaction_Surveys/CustomerSurvey> ;
                                                                                                      rdfs:comment "Instance for 'Customer Survey'" ;
                                                                                                      rdfs:label "Customer Survey Instance" .


###  http://www.semanticweb.org/alex/ontologies/2024/4/Flight_Satisfaction_Surveys/DomesticFlightInstance
<http://www.semanticweb.org/alex/ontologies/2024/4/Flight_Satisfaction_Surveys/DomesticFlightInstance> rdf:type owl:NamedIndividual ,
                                                                                                                <http://www.semanticweb.org/alex/ontologies/2024/4/Flight_Satisfaction_Surveys/DomesticFlight> ;
                                                                                                       rdfs:comment "Instance for 'Domestic Flight'" ;
                                                                                                       rdfs:label "Domestic Flight Instance" .


###  http://www.semanticweb.org/alex/ontologies/2024/4/Flight_Satisfaction_Surveys/FrequentFlyerInstance
<http://www.semanticweb.org/alex/ontologies/2024/4/Flight_Satisfaction_Surveys/FrequentFlyerInstance> rdf:type owl:NamedIndividual ,
                                                                                                               <http://www.semanticweb.org/alex/ontologies/2024/4/Flight_Satisfaction_Surveys/FrequentFlyer> ;
                                                                                                      rdfs:comment "Instance for 'Frequent Flyer'" ;
                                                                                                      rdfs:label "Frequent Flyer Instance" .


###  http://www.semanticweb.org/alex/ontologies/2024/4/Flight_Satisfaction_Surveys/InternationalFlightInstance
<http://www.semanticweb.org/alex/ontologies/2024/4/Flight_Satisfaction_Surveys/InternationalFlightInstance> rdf:type owl:NamedIndividual ,
                                                                                                                     <http://www.semanticweb.org/alex/ontologies/2024/4/Flight_Satisfaction_Surveys/InternationalFlight> ;
                                                                                                            rdfs:comment "Instance for 'International Flight'" ;
                                                                                                            rdfs:label "International Flight Instance" .


###  http://www.semanticweb.org/alex/ontologies/2024/4/Flight_Satisfaction_Surveys/LongHaulFlightInstance
<http://www.semanticweb.org/alex/ontologies/2024/4/Flight_Satisfaction_Surveys/LongHaulFlightInstance> rdf:type owl:NamedIndividual ,
                                                                                                                <http://www.semanticweb.org/alex/ontologies/2024/4/Flight_Satisfaction_Surveys/LongHaulFlight> ;
                                                                                                       rdfs:comment "Instance for 'Long Haul Flight'" ;
                                                                                                       rdfs:label "Long Haul Flight Instance" .


#################################################################
#    Rules
#################################################################

<urn:swrl:var#flight> rdf:type <http://www.w3.org/2003/11/swrl#Variable> .

<urn:swrl:var#duration> rdf:type <http://www.w3.org/2003/11/swrl#Variable> .

<urn:swrl:var#p> rdf:type <http://www.w3.org/2003/11/swrl#Variable> .

<urn:swrl:var#passenger> rdf:type <http://www.w3.org/2003/11/swrl#Variable> .

<urn:swrl:var#frequency> rdf:type <http://www.w3.org/2003/11/swrl#Variable> .

[ rdf:type <http://www.w3.org/2003/11/swrl#Imp> ;
   <http://www.w3.org/2003/11/swrl#body> [ rdf:type <http://www.w3.org/2003/11/swrl#AtomList> ;
                                           rdf:first [ rdf:type <http://www.w3.org/2003/11/swrl#ClassAtom> ;
                                                       <http://www.w3.org/2003/11/swrl#classPredicate> <http://www.semanticweb.org/alex/ontologies/2024/4/Flight_Satisfaction_Surveys/FlightDetails> ;
                                                       <http://www.w3.org/2003/11/swrl#argument1> <urn:swrl:var#flight>
                                                     ] ;
                                           rdf:rest [ rdf:type <http://www.w3.org/2003/11/swrl#AtomList> ;
                                                      rdf:first [ rdf:type <http://www.w3.org/2003/11/swrl#IndividualPropertyAtom> ;
                                                                  <http://www.w3.org/2003/11/swrl#propertyPredicate> <http://www.semanticweb.org/alex/ontologies/2024/4/Flight_Satisfaction_Surveys/hasFlightDuration> ;
                                                                  <http://www.w3.org/2003/11/swrl#argument1> <urn:swrl:var#flight> ;
                                                                  <http://www.w3.org/2003/11/swrl#argument2> <urn:swrl:var#duration>
                                                                ] ;
                                                      rdf:rest [ rdf:type <http://www.w3.org/2003/11/swrl#AtomList> ;
                                                                 rdf:first [ rdf:type <http://www.w3.org/2003/11/swrl#BuiltinAtom> ;
                                                                             <http://www.w3.org/2003/11/swrl#builtin> <http://www.w3.org/2003/11/swrlb#greaterThanOrEqual> ;
                                                                             <http://www.w3.org/2003/11/swrl#arguments> [ rdf:type rdf:List ;
                                                                                                                          rdf:first <urn:swrl:var#duration> ;
                                                                                                                          rdf:rest [ rdf:type rdf:List ;
                                                                                                                                     rdf:first 7 ;
                                                                                                                                     rdf:rest rdf:nil
                                                                                                                                   ]
                                                                                                                        ]
                                                                           ] ;
                                                                 rdf:rest rdf:nil
                                                               ]
                                                    ]
                                         ] ;
   <http://www.w3.org/2003/11/swrl#head> [ rdf:type <http://www.w3.org/2003/11/swrl#AtomList> ;
                                           rdf:first [ rdf:type <http://www.w3.org/2003/11/swrl#ClassAtom> ;
                                                       <http://www.w3.org/2003/11/swrl#classPredicate> <http://www.semanticweb.org/alex/ontologies/2024/4/Flight_Satisfaction_Surveys/LongHaulFlight> ;
                                                       <http://www.w3.org/2003/11/swrl#argument1> <urn:swrl:var#flight>
                                                     ] ;
                                           rdf:rest rdf:nil
                                         ]
 ] .

[ rdf:type <http://www.w3.org/2003/11/swrl#Imp> ;
   <http://www.w3.org/2003/11/swrl#body> [ rdf:type <http://www.w3.org/2003/11/swrl#AtomList> ;
                                           rdf:first [ rdf:type <http://www.w3.org/2003/11/swrl#ClassAtom> ;
                                                       <http://www.w3.org/2003/11/swrl#classPredicate> <http://www.semanticweb.org/alex/ontologies/2024/4/Flight_Satisfaction_Surveys/Passenger> ;
                                                       <http://www.w3.org/2003/11/swrl#argument1> <urn:swrl:var#p>
                                                     ] ;
                                           rdf:rest [ rdf:type <http://www.w3.org/2003/11/swrl#AtomList> ;
                                                      rdf:first [ rdf:type <http://www.w3.org/2003/11/swrl#ClassAtom> ;
                                                                  <http://www.w3.org/2003/11/swrl#classPredicate> <http://www.semanticweb.org/alex/ontologies/2024/4/Flight_Satisfaction_Surveys/FrequentFlyer> ;
                                                                  <http://www.w3.org/2003/11/swrl#argument1> <urn:swrl:var#p>
                                                                ] ;
                                                      rdf:rest rdf:nil
                                                    ]
                                         ] ;
   <http://www.w3.org/2003/11/swrl#head> [ rdf:type <http://www.w3.org/2003/11/swrl#AtomList> ;
                                           rdf:first [ rdf:type <http://www.w3.org/2003/11/swrl#ClassAtom> ;
                                                       <http://www.w3.org/2003/11/swrl#classPredicate> <http://www.semanticweb.org/alex/ontologies/2024/4/Flight_Satisfaction_Surveys/FrequentFlyer> ;
                                                       <http://www.w3.org/2003/11/swrl#argument1> <urn:swrl:var#p>
                                                     ] ;
                                           rdf:rest rdf:nil
                                         ]
 ] .

[ rdf:type <http://www.w3.org/2003/11/swrl#Imp> ;
   <http://www.w3.org/2003/11/swrl#body> [ rdf:type <http://www.w3.org/2003/11/swrl#AtomList> ;
                                           rdf:first [ rdf:type <http://www.w3.org/2003/11/swrl#ClassAtom> ;
                                                       <http://www.w3.org/2003/11/swrl#classPredicate> <http://www.semanticweb.org/alex/ontologies/2024/4/Flight_Satisfaction_Surveys/Passenger> ;
                                                       <http://www.w3.org/2003/11/swrl#argument1> <urn:swrl:var#passenger>
                                                     ] ;
                                           rdf:rest [ rdf:type <http://www.w3.org/2003/11/swrl#AtomList> ;
                                                      rdf:first [ rdf:type <http://www.w3.org/2003/11/swrl#ClassAtom> ;
                                                                  <http://www.w3.org/2003/11/swrl#classPredicate> <http://www.semanticweb.org/alex/ontologies/2024/4/Flight_Satisfaction_Surveys/FrequentFlyer> ;
                                                                  <http://www.w3.org/2003/11/swrl#argument1> <urn:swrl:var#passenger>
                                                                ] ;
                                                      rdf:rest [ rdf:type <http://www.w3.org/2003/11/swrl#AtomList> ;
                                                                 rdf:first [ rdf:type <http://www.w3.org/2003/11/swrl#IndividualPropertyAtom> ;
                                                                             <http://www.w3.org/2003/11/swrl#propertyPredicate> <http://www.semanticweb.org/alex/ontologies/2024/4/Flight_Satisfaction_Surveys/hasFlightFrequency> ;
                                                                             <http://www.w3.org/2003/11/swrl#argument1> <urn:swrl:var#passenger> ;
                                                                             <http://www.w3.org/2003/11/swrl#argument2> <urn:swrl:var#frequency>
                                                                           ] ;
                                                                 rdf:rest [ rdf:type <http://www.w3.org/2003/11/swrl#AtomList> ;
                                                                            rdf:first [ rdf:type <http://www.w3.org/2003/11/swrl#BuiltinAtom> ;
                                                                                        <http://www.w3.org/2003/11/swrl#builtin> <http://www.w3.org/2003/11/swrlb#greaterThanOrEqual> ;
                                                                                        <http://www.w3.org/2003/11/swrl#arguments> [ rdf:type rdf:List ;
                                                                                                                                     rdf:first <urn:swrl:var#frequency> ;
                                                                                                                                     rdf:rest [ rdf:type rdf:List ;
                                                                                                                                                rdf:first 100 ;
                                                                                                                                                rdf:rest rdf:nil
                                                                                                                                              ]
                                                                                                                                   ]
                                                                                      ] ;
                                                                            rdf:rest rdf:nil
                                                                          ]
                                                               ]
                                                    ]
                                         ] ;
   <http://www.w3.org/2003/11/swrl#head> [ rdf:type <http://www.w3.org/2003/11/swrl#AtomList> ;
                                           rdf:first [ rdf:type <http://www.w3.org/2003/11/swrl#ClassAtom> ;
                                                       <http://www.w3.org/2003/11/swrl#classPredicate> <http://www.semanticweb.org/alex/ontologies/2024/4/Flight_Satisfaction_Surveys/BusinessClassPassenger> ;
                                                       <http://www.w3.org/2003/11/swrl#argument1> <urn:swrl:var#passenger>
                                                     ] ;
                                           rdf:rest rdf:nil
                                         ]
 ] .

###  Generated by the OWL API (version 5.1.18) https://github.com/owlcs/owlapi/
