<?xml version="1.0"?>
<rdf:RDF xmlns="http://www.semanticweb.org/alex/ontologies/2024/4/Flight_Satisfaction_Surveys#"
     xml:base="http://www.semanticweb.org/alex/ontologies/2024/4/Flight_Satisfaction_Surveys"
     xmlns:owl="http://www.w3.org/2002/07/owl#"
     xmlns:rdf="http://www.w3.org/1999/02/22-rdf-syntax-ns#"
     xmlns:xml="http://www.w3.org/XML/1998/namespace"
     xmlns:xsd="http://www.w3.org/2001/XMLSchema#"
     xmlns:rdfs="http://www.w3.org/2000/01/rdf-schema#"
     xmlns:swrl="http://www.w3.org/2003/11/swrl#"
     xmlns:swrlb="http://www.w3.org/2003/11/swrlb#">
    <owl:Ontology rdf:about="http://www.semanticweb.org/alex/ontologies/2024/4/Flight_Satisfaction_Surveys">
        <rdfs:comment>@Author:
Alexander Vargas Pierola</rdfs:comment>
    </owl:Ontology>
    


    <!-- 
    ///////////////////////////////////////////////////////////////////////////////////////
    //
    // Annotation properties
    //
    ///////////////////////////////////////////////////////////////////////////////////////
     -->


    


    <!-- http://www.w3.org/2000/01/rdf-schema#comment -->


    <rdf:Description rdf:about="http://www.w3.org/2000/01/rdf-schema#comment">
        <rdfs:domain rdf:resource="http://www.semanticweb.org/alex/ontologies/2024/4/Flight_Satisfaction_Surveys/FlightSurvey"/>
    </rdf:Description>
    


    <!-- http://www.w3.org/2000/01/rdf-schema#sameAs -->


    <owl:AnnotationProperty rdf:about="http://www.w3.org/2000/01/rdf-schema#sameAs">
        <rdfs:subPropertyOf rdf:resource="http://www.w3.org/2000/01/rdf-schema#comment"/>
    </owl:AnnotationProperty>
    


    <!-- 
    ///////////////////////////////////////////////////////////////////////////////////////
    //
    // Object Properties
    //
    ///////////////////////////////////////////////////////////////////////////////////////
     -->


    


    <!-- http://www.semanticweb.org/alex/ontologies/2024/4/Flight_Satisfaction_Surveys/hasAirline -->


    <owl:ObjectProperty rdf:about="http://www.semanticweb.org/alex/ontologies/2024/4/Flight_Satisfaction_Surveys/hasAirline">
        <rdfs:domain rdf:resource="http://www.semanticweb.org/alex/ontologies/2024/4/Flight_Satisfaction_Surveys/FlightSurvey"/>
        <rdfs:range rdf:resource="http://www.semanticweb.org/alex/ontologies/2024/4/Flight_Satisfaction_Surveys/Airline"/>
        <rdfs:comment>Relates a flight survey to the airline associated with it.</rdfs:comment>
        <rdfs:label>has Airline</rdfs:label>
    </owl:ObjectProperty>
    


    <!-- http://www.semanticweb.org/alex/ontologies/2024/4/Flight_Satisfaction_Surveys/hasComment -->


    <owl:ObjectProperty rdf:about="http://www.semanticweb.org/alex/ontologies/2024/4/Flight_Satisfaction_Surveys/hasComment">
        <rdfs:domain rdf:resource="http://www.semanticweb.org/alex/ontologies/2024/4/Flight_Satisfaction_Surveys/FlightSurvey"/>
        <rdfs:range rdf:resource="http://www.semanticweb.org/alex/ontologies/2024/4/Flight_Satisfaction_Surveys/Passenger"/>
        <rdfs:label>has Comment</rdfs:label>
    </owl:ObjectProperty>
    


    <!-- http://www.semanticweb.org/alex/ontologies/2024/4/Flight_Satisfaction_Surveys/hasFlightDetails -->


    <owl:ObjectProperty rdf:about="http://www.semanticweb.org/alex/ontologies/2024/4/Flight_Satisfaction_Surveys/hasFlightDetails">
        <rdfs:domain rdf:resource="http://www.semanticweb.org/alex/ontologies/2024/4/Flight_Satisfaction_Surveys/FlightSurvey"/>
        <rdfs:range rdf:resource="http://www.semanticweb.org/alex/ontologies/2024/4/Flight_Satisfaction_Surveys/FlightDetails"/>
        <rdfs:comment>Relates a flight survey to the details of the flight it pertains to.</rdfs:comment>
        <rdfs:label>has Flight Details</rdfs:label>
    </owl:ObjectProperty>
    


    <!-- http://www.semanticweb.org/alex/ontologies/2024/4/Flight_Satisfaction_Surveys/hasFlightDuration -->


    <owl:ObjectProperty rdf:about="http://www.semanticweb.org/alex/ontologies/2024/4/Flight_Satisfaction_Surveys/hasFlightDuration">
        <rdfs:domain rdf:resource="http://www.semanticweb.org/alex/ontologies/2024/4/Flight_Satisfaction_Surveys/Airline"/>
        <rdfs:range rdf:resource="http://www.semanticweb.org/alex/ontologies/2024/4/Flight_Satisfaction_Surveys/FlightDetails"/>
        <rdfs:label>has Flight Duration</rdfs:label>
    </owl:ObjectProperty>
    


    <!-- http://www.semanticweb.org/alex/ontologies/2024/4/Flight_Satisfaction_Surveys/hasFlightFrequency -->


    <owl:ObjectProperty rdf:about="http://www.semanticweb.org/alex/ontologies/2024/4/Flight_Satisfaction_Surveys/hasFlightFrequency">
        <rdfs:domain rdf:resource="http://www.semanticweb.org/alex/ontologies/2024/4/Flight_Satisfaction_Surveys/Airline"/>
        <rdfs:range rdf:resource="http://www.semanticweb.org/alex/ontologies/2024/4/Flight_Satisfaction_Surveys/FlightDetails"/>
        <rdfs:label>has Flight Frequency</rdfs:label>
    </owl:ObjectProperty>
    


    <!-- http://www.semanticweb.org/alex/ontologies/2024/4/Flight_Satisfaction_Surveys/hasPassenger -->


    <owl:ObjectProperty rdf:about="http://www.semanticweb.org/alex/ontologies/2024/4/Flight_Satisfaction_Surveys/hasPassenger">
        <rdfs:domain rdf:resource="http://www.semanticweb.org/alex/ontologies/2024/4/Flight_Satisfaction_Surveys/FlightSurvey"/>
        <rdfs:range rdf:resource="http://www.semanticweb.org/alex/ontologies/2024/4/Flight_Satisfaction_Surveys/Passenger"/>
        <rdfs:comment>Relates a flight survey to the passenger who participated in it.</rdfs:comment>
        <rdfs:label>has Passenger</rdfs:label>
    </owl:ObjectProperty>
    


    <!-- 
    ///////////////////////////////////////////////////////////////////////////////////////
    //
    // Data properties
    //
    ///////////////////////////////////////////////////////////////////////////////////////
     -->


    


    <!-- http://www.semanticweb.org/alex/ontologies/2024/4/Flight_Satisfaction_Surveys/Aircraft -->


    <owl:DatatypeProperty rdf:about="http://www.semanticweb.org/alex/ontologies/2024/4/Flight_Satisfaction_Surveys/Aircraft">
        <rdfs:subPropertyOf rdf:resource="http://www.w3.org/2002/07/owl#topDataProperty"/>
        <rdfs:domain rdf:resource="http://www.semanticweb.org/alex/ontologies/2024/4/Flight_Satisfaction_Surveys/FlightDetails"/>
        <rdfs:range rdf:resource="http://www.w3.org/2001/XMLSchema#string"/>
        <rdfs:comment>The type or model of the aircraft used for the flight.</rdfs:comment>
        <rdfs:label>Aircraft</rdfs:label>
    </owl:DatatypeProperty>
    


    <!-- http://www.semanticweb.org/alex/ontologies/2024/4/Flight_Satisfaction_Surveys/CabinStaffService -->


    <owl:DatatypeProperty rdf:about="http://www.semanticweb.org/alex/ontologies/2024/4/Flight_Satisfaction_Surveys/CabinStaffService">
        <rdfs:subPropertyOf rdf:resource="http://www.w3.org/2002/07/owl#topDataProperty"/>
        <rdfs:domain rdf:resource="http://www.semanticweb.org/alex/ontologies/2024/4/Flight_Satisfaction_Surveys/FlightSurvey"/>
        <rdfs:range rdf:resource="http://www.w3.org/2001/XMLSchema#integer"/>
        <rdfs:comment>The rating or score given by the passenger for the service provided by the cabin staff.</rdfs:comment>
        <rdfs:label>Cabin Staff Service</rdfs:label>
    </owl:DatatypeProperty>
    


    <!-- http://www.semanticweb.org/alex/ontologies/2024/4/Flight_Satisfaction_Surveys/Comment -->


    <owl:DatatypeProperty rdf:about="http://www.semanticweb.org/alex/ontologies/2024/4/Flight_Satisfaction_Surveys/Comment">
        <rdfs:subPropertyOf rdf:resource="http://www.w3.org/2002/07/owl#topDataProperty"/>
        <rdfs:domain rdf:resource="http://www.semanticweb.org/alex/ontologies/2024/4/Flight_Satisfaction_Surveys/FlightSurvey"/>
        <rdfs:range rdf:resource="http://www.w3.org/2001/XMLSchema#string"/>
        <rdfs:comment>The detailed comment provided by the passenger about their flight experience.</rdfs:comment>
        <rdfs:label>Comment</rdfs:label>
    </owl:DatatypeProperty>
    


    <!-- http://www.semanticweb.org/alex/ontologies/2024/4/Flight_Satisfaction_Surveys/CommentTitle -->


    <owl:DatatypeProperty rdf:about="http://www.semanticweb.org/alex/ontologies/2024/4/Flight_Satisfaction_Surveys/CommentTitle">
        <rdfs:subPropertyOf rdf:resource="http://www.w3.org/2002/07/owl#topDataProperty"/>
        <rdfs:domain rdf:resource="http://www.semanticweb.org/alex/ontologies/2024/4/Flight_Satisfaction_Surveys/FlightSurvey"/>
        <rdfs:range rdf:resource="http://www.w3.org/2001/XMLSchema#string"/>
        <rdfs:comment>The title of the passenger&apos;s comment about their flight experience.</rdfs:comment>
        <rdfs:label>Comment Title</rdfs:label>
    </owl:DatatypeProperty>
    


    <!-- http://www.semanticweb.org/alex/ontologies/2024/4/Flight_Satisfaction_Surveys/DateFlown -->


    <owl:DatatypeProperty rdf:about="http://www.semanticweb.org/alex/ontologies/2024/4/Flight_Satisfaction_Surveys/DateFlown">
        <rdfs:subPropertyOf rdf:resource="http://www.w3.org/2002/07/owl#topDataProperty"/>
        <rdfs:domain rdf:resource="http://www.semanticweb.org/alex/ontologies/2024/4/Flight_Satisfaction_Surveys/FlightDetails"/>
        <rdfs:range rdf:resource="http://www.w3.org/2001/XMLSchema#dateTime"/>
        <rdfs:comment>The date when the flight was taken or flown.</rdfs:comment>
        <rdfs:label>Date Flown</rdfs:label>
    </owl:DatatypeProperty>
    


    <!-- http://www.semanticweb.org/alex/ontologies/2024/4/Flight_Satisfaction_Surveys/DatePublished -->


    <owl:DatatypeProperty rdf:about="http://www.semanticweb.org/alex/ontologies/2024/4/Flight_Satisfaction_Surveys/DatePublished">
        <rdfs:subPropertyOf rdf:resource="http://www.w3.org/2002/07/owl#topDataProperty"/>
        <rdfs:domain rdf:resource="http://www.semanticweb.org/alex/ontologies/2024/4/Flight_Satisfaction_Surveys/FlightSurvey"/>
        <rdfs:range rdf:resource="http://www.w3.org/2001/XMLSchema#dateTime"/>
        <rdfs:comment>The date when the flight survey was published or made available.</rdfs:comment>
        <rdfs:label>Date Published</rdfs:label>
    </owl:DatatypeProperty>
    


    <!-- http://www.semanticweb.org/alex/ontologies/2024/4/Flight_Satisfaction_Surveys/Destination -->


    <owl:DatatypeProperty rdf:about="http://www.semanticweb.org/alex/ontologies/2024/4/Flight_Satisfaction_Surveys/Destination">
        <rdfs:subPropertyOf rdf:resource="http://www.w3.org/2002/07/owl#topDataProperty"/>
        <rdfs:domain rdf:resource="http://www.semanticweb.org/alex/ontologies/2024/4/Flight_Satisfaction_Surveys/FlightDetails"/>
        <rdfs:range rdf:resource="http://www.w3.org/2001/XMLSchema#string"/>
        <rdfs:comment>The arrival location or destination of the flight.</rdfs:comment>
        <rdfs:label>Destination</rdfs:label>
    </owl:DatatypeProperty>
    


    <!-- http://www.semanticweb.org/alex/ontologies/2024/4/Flight_Satisfaction_Surveys/FoodAndBeverages -->


    <owl:DatatypeProperty rdf:about="http://www.semanticweb.org/alex/ontologies/2024/4/Flight_Satisfaction_Surveys/FoodAndBeverages">
        <rdfs:subPropertyOf rdf:resource="http://www.w3.org/2002/07/owl#topDataProperty"/>
        <rdfs:domain rdf:resource="http://www.semanticweb.org/alex/ontologies/2024/4/Flight_Satisfaction_Surveys/FlightSurvey"/>
        <rdfs:range rdf:resource="http://www.w3.org/2001/XMLSchema#integer"/>
        <rdfs:comment>The rating or score given by the passenger for the quality of food and beverages provided during the flight.</rdfs:comment>
        <rdfs:label>Food And Beverages</rdfs:label>
    </owl:DatatypeProperty>
    


    <!-- http://www.semanticweb.org/alex/ontologies/2024/4/Flight_Satisfaction_Surveys/GroundService -->


    <owl:DatatypeProperty rdf:about="http://www.semanticweb.org/alex/ontologies/2024/4/Flight_Satisfaction_Surveys/GroundService">
        <rdfs:subPropertyOf rdf:resource="http://www.w3.org/2002/07/owl#topDataProperty"/>
        <rdfs:domain rdf:resource="http://www.semanticweb.org/alex/ontologies/2024/4/Flight_Satisfaction_Surveys/FlightSurvey"/>
        <rdfs:range rdf:resource="http://www.w3.org/2001/XMLSchema#integer"/>
        <rdfs:comment>The rating or score given by the passenger for the ground services provided at the airport.</rdfs:comment>
        <rdfs:label>Ground Service</rdfs:label>
    </owl:DatatypeProperty>
    


    <!-- http://www.semanticweb.org/alex/ontologies/2024/4/Flight_Satisfaction_Surveys/InflightEntertainment -->


    <owl:DatatypeProperty rdf:about="http://www.semanticweb.org/alex/ontologies/2024/4/Flight_Satisfaction_Surveys/InflightEntertainment">
        <rdfs:subPropertyOf rdf:resource="http://www.w3.org/2002/07/owl#topDataProperty"/>
        <rdfs:domain rdf:resource="http://www.semanticweb.org/alex/ontologies/2024/4/Flight_Satisfaction_Surveys/FlightSurvey"/>
        <rdfs:range rdf:resource="http://www.w3.org/2001/XMLSchema#integer"/>
        <rdfs:comment>The rating or score given by the passenger for the quality of inflight entertainment options.</rdfs:comment>
        <rdfs:label>Inflight Entertainment</rdfs:label>
    </owl:DatatypeProperty>
    


    <!-- http://www.semanticweb.org/alex/ontologies/2024/4/Flight_Satisfaction_Surveys/Origin -->


    <owl:DatatypeProperty rdf:about="http://www.semanticweb.org/alex/ontologies/2024/4/Flight_Satisfaction_Surveys/Origin">
        <rdfs:subPropertyOf rdf:resource="http://www.w3.org/2002/07/owl#topDataProperty"/>
        <rdfs:domain rdf:resource="http://www.semanticweb.org/alex/ontologies/2024/4/Flight_Satisfaction_Surveys/FlightDetails"/>
        <rdfs:range rdf:resource="http://www.w3.org/2001/XMLSchema#string"/>
        <rdfs:comment>The departure location or origin of the flight.</rdfs:comment>
        <rdfs:label>Origin</rdfs:label>
    </owl:DatatypeProperty>
    


    <!-- http://www.semanticweb.org/alex/ontologies/2024/4/Flight_Satisfaction_Surveys/OverallRating -->


    <owl:DatatypeProperty rdf:about="http://www.semanticweb.org/alex/ontologies/2024/4/Flight_Satisfaction_Surveys/OverallRating">
        <rdfs:subPropertyOf rdf:resource="http://www.w3.org/2002/07/owl#topDataProperty"/>
        <rdfs:domain rdf:resource="http://www.semanticweb.org/alex/ontologies/2024/4/Flight_Satisfaction_Surveys/FlightSurvey"/>
        <rdfs:range>
            <rdfs:Datatype>
                <owl:onDatatype rdf:resource="http://www.w3.org/2001/XMLSchema#integer"/>
                <owl:withRestrictions rdf:parseType="Collection">
                    <rdf:Description>
                        <xsd:minInclusive rdf:datatype="http://www.w3.org/2001/XMLSchema#integer">1</xsd:minInclusive>
                    </rdf:Description>
                    <rdf:Description>
                        <xsd:maxInclusive rdf:datatype="http://www.w3.org/2001/XMLSchema#integer">10</xsd:maxInclusive>
                    </rdf:Description>
                </owl:withRestrictions>
            </rdfs:Datatype>
        </rdfs:range>
        <rdfs:comment>The overall rating or score given by the passenger for their flight experience.</rdfs:comment>
        <rdfs:label>Overall Rating</rdfs:label>
    </owl:DatatypeProperty>
    


    <!-- http://www.semanticweb.org/alex/ontologies/2024/4/Flight_Satisfaction_Surveys/PassengerCountry -->


    <owl:DatatypeProperty rdf:about="http://www.semanticweb.org/alex/ontologies/2024/4/Flight_Satisfaction_Surveys/PassengerCountry">
        <rdfs:subPropertyOf rdf:resource="http://www.w3.org/2002/07/owl#topDataProperty"/>
        <rdfs:domain rdf:resource="http://www.semanticweb.org/alex/ontologies/2024/4/Flight_Satisfaction_Surveys/Passenger"/>
        <rdfs:range rdf:resource="http://www.w3.org/2001/XMLSchema#string"/>
        <rdfs:comment>The country of origin of the passenger.</rdfs:comment>
        <rdfs:label>Passenger Country</rdfs:label>
    </owl:DatatypeProperty>
    


    <!-- http://www.semanticweb.org/alex/ontologies/2024/4/Flight_Satisfaction_Surveys/Recommended -->


    <owl:DatatypeProperty rdf:about="http://www.semanticweb.org/alex/ontologies/2024/4/Flight_Satisfaction_Surveys/Recommended">
        <rdfs:subPropertyOf rdf:resource="http://www.w3.org/2002/07/owl#topDataProperty"/>
        <rdfs:domain rdf:resource="http://www.semanticweb.org/alex/ontologies/2024/4/Flight_Satisfaction_Surveys/FlightSurvey"/>
        <rdfs:range>
            <rdfs:Datatype>
                <owl:oneOf>
                    <rdf:Description>
                        <rdf:type rdf:resource="http://www.w3.org/1999/02/22-rdf-syntax-ns#List"/>
                        <rdf:first>no</rdf:first>
                        <rdf:rest>
                            <rdf:Description>
                                <rdf:type rdf:resource="http://www.w3.org/1999/02/22-rdf-syntax-ns#List"/>
                                <rdf:first>yes</rdf:first>
                                <rdf:rest rdf:resource="http://www.w3.org/1999/02/22-rdf-syntax-ns#nil"/>
                            </rdf:Description>
                        </rdf:rest>
                    </rdf:Description>
                </owl:oneOf>
            </rdfs:Datatype>
        </rdfs:range>
        <rdfs:comment>Indicates whether the passenger would recommend the airline or flight to others</rdfs:comment>
        <rdfs:label>Recommended</rdfs:label>
    </owl:DatatypeProperty>
    


    <!-- http://www.semanticweb.org/alex/ontologies/2024/4/Flight_Satisfaction_Surveys/SeatComfort -->


    <owl:DatatypeProperty rdf:about="http://www.semanticweb.org/alex/ontologies/2024/4/Flight_Satisfaction_Surveys/SeatComfort">
        <rdfs:subPropertyOf rdf:resource="http://www.w3.org/2002/07/owl#topDataProperty"/>
        <rdfs:domain rdf:resource="http://www.semanticweb.org/alex/ontologies/2024/4/Flight_Satisfaction_Surveys/FlightSurvey"/>
        <rdfs:range rdf:resource="http://www.w3.org/2001/XMLSchema#integer"/>
        <rdfs:comment>The rating or score given by the passenger for the comfort of the seating arrangement.</rdfs:comment>
        <rdfs:label>Seat Comfort</rdfs:label>
    </owl:DatatypeProperty>
    


    <!-- http://www.semanticweb.org/alex/ontologies/2024/4/Flight_Satisfaction_Surveys/SeatType -->


    <owl:DatatypeProperty rdf:about="http://www.semanticweb.org/alex/ontologies/2024/4/Flight_Satisfaction_Surveys/SeatType">
        <rdfs:subPropertyOf rdf:resource="http://www.w3.org/2002/07/owl#topDataProperty"/>
        <rdfs:domain rdf:resource="http://www.semanticweb.org/alex/ontologies/2024/4/Flight_Satisfaction_Surveys/FlightDetails"/>
        <rdfs:range rdf:resource="http://www.w3.org/2001/XMLSchema#string"/>
        <rdfs:comment>The type or class of seating arrangement on the flight, for example economy, business, etc.</rdfs:comment>
        <rdfs:label>Seat Type</rdfs:label>
    </owl:DatatypeProperty>
    


    <!-- http://www.semanticweb.org/alex/ontologies/2024/4/Flight_Satisfaction_Surveys/TripVerified -->


    <owl:DatatypeProperty rdf:about="http://www.semanticweb.org/alex/ontologies/2024/4/Flight_Satisfaction_Surveys/TripVerified">
        <rdfs:subPropertyOf rdf:resource="http://www.w3.org/2002/07/owl#topDataProperty"/>
        <rdfs:domain rdf:resource="http://www.semanticweb.org/alex/ontologies/2024/4/Flight_Satisfaction_Surveys/FlightDetails"/>
        <rdfs:range rdf:resource="http://www.w3.org/2001/XMLSchema#string"/>
        <rdfs:comment>Indicates whether the trip details have been verified by the passenger.</rdfs:comment>
        <rdfs:label>Trip Verified</rdfs:label>
    </owl:DatatypeProperty>
    


    <!-- http://www.semanticweb.org/alex/ontologies/2024/4/Flight_Satisfaction_Surveys/TypeOfTraveller -->


    <owl:DatatypeProperty rdf:about="http://www.semanticweb.org/alex/ontologies/2024/4/Flight_Satisfaction_Surveys/TypeOfTraveller">
        <rdfs:subPropertyOf rdf:resource="http://www.w3.org/2002/07/owl#topDataProperty"/>
        <rdfs:domain rdf:resource="http://www.semanticweb.org/alex/ontologies/2024/4/Flight_Satisfaction_Surveys/Passenger"/>
        <rdfs:range rdf:resource="http://www.w3.org/2001/XMLSchema#string"/>
        <rdfs:comment>The type or category of the passenger, for example business traveler, leisure traveler, etc.</rdfs:comment>
        <rdfs:label>Type Of Traveller</rdfs:label>
    </owl:DatatypeProperty>
    


    <!-- http://www.semanticweb.org/alex/ontologies/2024/4/Flight_Satisfaction_Surveys/ValueForMoney -->


    <owl:DatatypeProperty rdf:about="http://www.semanticweb.org/alex/ontologies/2024/4/Flight_Satisfaction_Surveys/ValueForMoney">
        <rdfs:subPropertyOf rdf:resource="http://www.w3.org/2002/07/owl#topDataProperty"/>
        <rdfs:domain rdf:resource="http://www.semanticweb.org/alex/ontologies/2024/4/Flight_Satisfaction_Surveys/FlightSurvey"/>
        <rdfs:range rdf:resource="http://www.w3.org/2001/XMLSchema#integer"/>
        <rdfs:comment>The rating or score given by the passenger for the perceived value for money of the flight experience.</rdfs:comment>
        <rdfs:label>Value For Money</rdfs:label>
    </owl:DatatypeProperty>
    


    <!-- http://www.semanticweb.org/alex/ontologies/2024/4/Flight_Satisfaction_Surveys/WifiAndConnectivity -->


    <owl:DatatypeProperty rdf:about="http://www.semanticweb.org/alex/ontologies/2024/4/Flight_Satisfaction_Surveys/WifiAndConnectivity">
        <rdfs:subPropertyOf rdf:resource="http://www.w3.org/2002/07/owl#topDataProperty"/>
        <rdfs:domain rdf:resource="http://www.semanticweb.org/alex/ontologies/2024/4/Flight_Satisfaction_Surveys/FlightSurvey"/>
        <rdfs:range rdf:resource="http://www.w3.org/2001/XMLSchema#integer"/>
        <rdfs:label>The rating or score given by the passenger for the quality of Wi-Fi and connectivity services were available during the flight.</rdfs:label>
        <rdfs:label>Wifi And Connectivity</rdfs:label>
    </owl:DatatypeProperty>
    


    <!-- 
    ///////////////////////////////////////////////////////////////////////////////////////
    //
    // Classes
    //
    ///////////////////////////////////////////////////////////////////////////////////////
     -->


    


    <!-- http://www.semanticweb.org/alex/ontologies/2024/4/Flight_Satisfaction_Surveys/Airline -->


    <owl:Class rdf:about="http://www.semanticweb.org/alex/ontologies/2024/4/Flight_Satisfaction_Surveys/Airline">
        <rdfs:comment>Represents an airline company providing flight services to passengers.</rdfs:comment>
        <rdfs:label>Airline</rdfs:label>
    </owl:Class>
    


    <!-- http://www.semanticweb.org/alex/ontologies/2024/4/Flight_Satisfaction_Surveys/ArrivalExperienceSurvey -->


    <owl:Class rdf:about="http://www.semanticweb.org/alex/ontologies/2024/4/Flight_Satisfaction_Surveys/ArrivalExperienceSurvey">
        <rdfs:subClassOf rdf:resource="http://www.semanticweb.org/alex/ontologies/2024/4/Flight_Satisfaction_Surveys/PostFlightSurvey"/>
        <rdfs:comment>Represents a survey used to gather feedback from passengers about their experience upon arrival at the destination airport, including customs, immigration, and ground transportation.</rdfs:comment>
        <rdfs:label>Arrival Experience Survey</rdfs:label>
    </owl:Class>
    


    <!-- http://www.semanticweb.org/alex/ontologies/2024/4/Flight_Satisfaction_Surveys/BaggageClaimSurvey -->


    <owl:Class rdf:about="http://www.semanticweb.org/alex/ontologies/2024/4/Flight_Satisfaction_Surveys/BaggageClaimSurvey">
        <rdfs:subClassOf rdf:resource="http://www.semanticweb.org/alex/ontologies/2024/4/Flight_Satisfaction_Surveys/PostFlightSurvey"/>
        <rdfs:comment>Represents a survey used to gather feedback from passengers about their experience at the baggage claim area, including the efficiency and convenience of baggage retrieval.</rdfs:comment>
        <rdfs:label>Baggage Claim Survey</rdfs:label>
    </owl:Class>
    


    <!-- http://www.semanticweb.org/alex/ontologies/2024/4/Flight_Satisfaction_Surveys/BasicEconomyClassPassenger -->


    <owl:Class rdf:about="http://www.semanticweb.org/alex/ontologies/2024/4/Flight_Satisfaction_Surveys/BasicEconomyClassPassenger">
        <rdfs:subClassOf rdf:resource="http://www.semanticweb.org/alex/ontologies/2024/4/Flight_Satisfaction_Surveys/EconomyClassPassenger"/>
        <rdfs:comment>Represents a passenger traveling in the basic or standard economy class cabin of an aircraft, offering essential amenities and services at a lower cost.</rdfs:comment>
        <rdfs:label>Basic Economy Class Passenger</rdfs:label>
    </owl:Class>
    


    <!-- http://www.semanticweb.org/alex/ontologies/2024/4/Flight_Satisfaction_Surveys/BusinessClassPassenger -->


    <owl:Class rdf:about="http://www.semanticweb.org/alex/ontologies/2024/4/Flight_Satisfaction_Surveys/BusinessClassPassenger">
        <rdfs:subClassOf rdf:resource="http://www.semanticweb.org/alex/ontologies/2024/4/Flight_Satisfaction_Surveys/Passenger"/>
        <rdfs:comment>Represents a passenger who travels in the business class cabin of an aircraft, normally offering enhanced amenities and services compared to economy class.</rdfs:comment>
        <rdfs:label>Business Class Passenger</rdfs:label>
        <rdfs:sameAs>http://dbpedia.org/resource/Business_class</rdfs:sameAs>
    </owl:Class>
    


    <!-- http://www.semanticweb.org/alex/ontologies/2024/4/Flight_Satisfaction_Surveys/CrewSatisfactionSurvey -->


    <owl:Class rdf:about="http://www.semanticweb.org/alex/ontologies/2024/4/Flight_Satisfaction_Surveys/CrewSatisfactionSurvey">
        <rdfs:subClassOf rdf:resource="http://www.semanticweb.org/alex/ontologies/2024/4/Flight_Satisfaction_Surveys/EmployeeSurvey"/>
        <rdfs:comment>Represents a survey conducted to gather feedback from airline crew members about their job satisfaction, working conditions, and overall experience in their roles.</rdfs:comment>
        <rdfs:label>Crew Satisfaction Survey</rdfs:label>
    </owl:Class>
    


    <!-- http://www.semanticweb.org/alex/ontologies/2024/4/Flight_Satisfaction_Surveys/CustomerSurvey -->


    <owl:Class rdf:about="http://www.semanticweb.org/alex/ontologies/2024/4/Flight_Satisfaction_Surveys/CustomerSurvey">
        <rdfs:subClassOf rdf:resource="http://www.semanticweb.org/alex/ontologies/2024/4/Flight_Satisfaction_Surveys/FlightSurvey"/>
        <rdfs:comment>Represents a survey used to gather feedback from customers about their experience with a product or service.</rdfs:comment>
        <rdfs:label>Customer Survey</rdfs:label>
    </owl:Class>
    


    <!-- http://www.semanticweb.org/alex/ontologies/2024/4/Flight_Satisfaction_Surveys/DomesticFlight -->


    <owl:Class rdf:about="http://www.semanticweb.org/alex/ontologies/2024/4/Flight_Satisfaction_Surveys/DomesticFlight">
        <rdfs:subClassOf rdf:resource="http://www.semanticweb.org/alex/ontologies/2024/4/Flight_Satisfaction_Surveys/Airline"/>
        <rdfs:comment>Represents a flight that operates within the borders of a single country, without crossing international boundaries.</rdfs:comment>
        <rdfs:label>Domestic Flight</rdfs:label>
    </owl:Class>
    


    <!-- http://www.semanticweb.org/alex/ontologies/2024/4/Flight_Satisfaction_Surveys/DomesticLongHaulFlight -->


    <owl:Class rdf:about="http://www.semanticweb.org/alex/ontologies/2024/4/Flight_Satisfaction_Surveys/DomesticLongHaulFlight">
        <rdfs:subClassOf rdf:resource="http://www.semanticweb.org/alex/ontologies/2024/4/Flight_Satisfaction_Surveys/LongHaulFlight"/>
        <rdfs:comment>Represents a long-haul flight operating within a country or region, covering extensive distances.</rdfs:comment>
        <rdfs:label>Domestic Long Haul Flight</rdfs:label>
    </owl:Class>
    


    <!-- http://www.semanticweb.org/alex/ontologies/2024/4/Flight_Satisfaction_Surveys/DomesticRegionalAirline -->


    <owl:Class rdf:about="http://www.semanticweb.org/alex/ontologies/2024/4/Flight_Satisfaction_Surveys/DomesticRegionalAirline">
        <rdfs:subClassOf rdf:resource="http://www.semanticweb.org/alex/ontologies/2024/4/Flight_Satisfaction_Surveys/RegionalAirline"/>
        <rdfs:comment>Represents a regional airline specializing in offering flight services within a specific country or region.</rdfs:comment>
        <rdfs:label>Domestic Regional Airline</rdfs:label>
    </owl:Class>
    


    <!-- http://www.semanticweb.org/alex/ontologies/2024/4/Flight_Satisfaction_Surveys/EconomyClassPassenger -->


    <owl:Class rdf:about="http://www.semanticweb.org/alex/ontologies/2024/4/Flight_Satisfaction_Surveys/EconomyClassPassenger">
        <rdfs:subClassOf rdf:resource="http://www.semanticweb.org/alex/ontologies/2024/4/Flight_Satisfaction_Surveys/Passenger"/>
        <rdfs:comment>Represents a passenger who travels in the economy class cabin of an aircraft, normally offering standard amenities and services.</rdfs:comment>
        <rdfs:label>Economy Class Passenger</rdfs:label>
    </owl:Class>
    


    <!-- http://www.semanticweb.org/alex/ontologies/2024/4/Flight_Satisfaction_Surveys/EliteFrequentFlyer -->


    <owl:Class rdf:about="http://www.semanticweb.org/alex/ontologies/2024/4/Flight_Satisfaction_Surveys/EliteFrequentFlyer">
        <rdfs:subClassOf rdf:resource="http://www.semanticweb.org/alex/ontologies/2024/4/Flight_Satisfaction_Surveys/FrequentFlyer"/>
        <rdfs:comment>Represents a frequent flyer with elite status in an airline&apos;s loyalty program, enjoying exclusive benefits, privileges, and rewards.</rdfs:comment>
        <rdfs:label>Elite Frequent Flyer</rdfs:label>
    </owl:Class>
    


    <!-- http://www.semanticweb.org/alex/ontologies/2024/4/Flight_Satisfaction_Surveys/EmployeeSurvey -->


    <owl:Class rdf:about="http://www.semanticweb.org/alex/ontologies/2024/4/Flight_Satisfaction_Surveys/EmployeeSurvey">
        <rdfs:subClassOf rdf:resource="http://www.semanticweb.org/alex/ontologies/2024/4/Flight_Satisfaction_Surveys/FlightSurvey"/>
        <rdfs:comment>Represents a survey used to gather feedback from employees about their job satisfaction, work environment, and other related aspects.</rdfs:comment>
        <rdfs:label>Employee Survey</rdfs:label>
    </owl:Class>
    


    <!-- http://www.semanticweb.org/alex/ontologies/2024/4/Flight_Satisfaction_Surveys/ExperienceSurvey -->


    <owl:Class rdf:about="http://www.semanticweb.org/alex/ontologies/2024/4/Flight_Satisfaction_Surveys/ExperienceSurvey">
        <rdfs:subClassOf rdf:resource="http://www.semanticweb.org/alex/ontologies/2024/4/Flight_Satisfaction_Surveys/CustomerSurvey"/>
        <rdfs:comment>Represents a survey designed to gather feedback from customers about their overall experience, including interactions, perceptions, and sentiments.</rdfs:comment>
        <rdfs:label>Experience Survey</rdfs:label>
    </owl:Class>
    


    <!-- http://www.semanticweb.org/alex/ontologies/2024/4/Flight_Satisfaction_Surveys/FamilyLeisureTraveler -->


    <owl:Class rdf:about="http://www.semanticweb.org/alex/ontologies/2024/4/Flight_Satisfaction_Surveys/FamilyLeisureTraveler">
        <rdfs:subClassOf rdf:resource="http://www.semanticweb.org/alex/ontologies/2024/4/Flight_Satisfaction_Surveys/LeisureTraveler"/>
        <rdfs:comment>Represents a leisure traveler who travels with family members for vacation, holidays, or recreational activities, often seeking family-friendly travel options.</rdfs:comment>
        <rdfs:label>Family Leisure Traveler</rdfs:label>
    </owl:Class>
    


    <!-- http://www.semanticweb.org/alex/ontologies/2024/4/Flight_Satisfaction_Surveys/FlightDetails -->


    <owl:Class rdf:about="http://www.semanticweb.org/alex/ontologies/2024/4/Flight_Satisfaction_Surveys/FlightDetails">
        <rdfs:comment>Represents the specific details of a flight, including its route, duration, and the main information.</rdfs:comment>
        <rdfs:label>Flight Details</rdfs:label>
    </owl:Class>
    


    <!-- http://www.semanticweb.org/alex/ontologies/2024/4/Flight_Satisfaction_Surveys/FlightSurvey -->


    <owl:Class rdf:about="http://www.semanticweb.org/alex/ontologies/2024/4/Flight_Satisfaction_Surveys/FlightSurvey">
        <rdfs:subClassOf>
            <owl:Restriction>
                <owl:onProperty rdf:resource="http://www.semanticweb.org/alex/ontologies/2024/4/Flight_Satisfaction_Surveys/hasAirline"/>
                <owl:qualifiedCardinality rdf:datatype="http://www.w3.org/2001/XMLSchema#nonNegativeInteger">1</owl:qualifiedCardinality>
                <owl:onClass rdf:resource="http://www.semanticweb.org/alex/ontologies/2024/4/Flight_Satisfaction_Surveys/FlightSurvey"/>
            </owl:Restriction>
        </rdfs:subClassOf>
        <rdfs:subClassOf>
            <owl:Restriction>
                <owl:onProperty rdf:resource="http://www.semanticweb.org/alex/ontologies/2024/4/Flight_Satisfaction_Surveys/hasPassenger"/>
                <owl:qualifiedCardinality rdf:datatype="http://www.w3.org/2001/XMLSchema#nonNegativeInteger">1</owl:qualifiedCardinality>
                <owl:onClass rdf:resource="http://www.semanticweb.org/alex/ontologies/2024/4/Flight_Satisfaction_Surveys/FlightSurvey"/>
            </owl:Restriction>
        </rdfs:subClassOf>
        <rdfs:subClassOf>
            <owl:Restriction>
                <owl:onProperty rdf:resource="http://www.semanticweb.org/alex/ontologies/2024/4/Flight_Satisfaction_Surveys/hasFlightDetails"/>
                <owl:maxQualifiedCardinality rdf:datatype="http://www.w3.org/2001/XMLSchema#nonNegativeInteger">1</owl:maxQualifiedCardinality>
                <owl:onClass rdf:resource="http://www.semanticweb.org/alex/ontologies/2024/4/Flight_Satisfaction_Surveys/FlightSurvey"/>
            </owl:Restriction>
        </rdfs:subClassOf>
        <rdfs:comment>Represents a survey used to gather feedback from different people about their flight experience.</rdfs:comment>
        <rdfs:label>Flight Survey</rdfs:label>
    </owl:Class>
    


    <!-- http://www.semanticweb.org/alex/ontologies/2024/4/Flight_Satisfaction_Surveys/FrequentFlyer -->


    <owl:Class rdf:about="http://www.semanticweb.org/alex/ontologies/2024/4/Flight_Satisfaction_Surveys/FrequentFlyer">
        <rdfs:subClassOf rdf:resource="http://www.semanticweb.org/alex/ontologies/2024/4/Flight_Satisfaction_Surveys/Passenger"/>
        <rdfs:comment>Represents a passenger who frequently travels by air and may be enrolled in a loyalty program offered by an airline.</rdfs:comment>
        <rdfs:label>Frequent Flyer</rdfs:label>
    </owl:Class>
    


    <!-- http://www.semanticweb.org/alex/ontologies/2024/4/Flight_Satisfaction_Surveys/FullServiceInternationalAirline -->


    <owl:Class rdf:about="http://www.semanticweb.org/alex/ontologies/2024/4/Flight_Satisfaction_Surveys/FullServiceInternationalAirline">
        <rdfs:subClassOf rdf:resource="http://www.semanticweb.org/alex/ontologies/2024/4/Flight_Satisfaction_Surveys/InternationalAirline"/>
        <rdfs:comment>Represents an international airline company that offers comprehensive flight services, including various cabin classes, amenities, and customer services.</rdfs:comment>
        <rdfs:label>Full Service International Airline</rdfs:label>
    </owl:Class>
    


    <!-- http://www.semanticweb.org/alex/ontologies/2024/4/Flight_Satisfaction_Surveys/GroundStaffSurvey -->


    <owl:Class rdf:about="http://www.semanticweb.org/alex/ontologies/2024/4/Flight_Satisfaction_Surveys/GroundStaffSurvey">
        <rdfs:subClassOf rdf:resource="http://www.semanticweb.org/alex/ontologies/2024/4/Flight_Satisfaction_Surveys/EmployeeSurvey"/>
        <rdfs:comment>Ground Staff Survey</rdfs:comment>
        <rdfs:comment>Represents a survey used to gather feedback from ground staff employees, such as airport personnel and support staff, about their job satisfaction and work environment.</rdfs:comment>
    </owl:Class>
    


    <!-- http://www.semanticweb.org/alex/ontologies/2024/4/Flight_Satisfaction_Surveys/HybridInternationalAirline -->


    <owl:Class rdf:about="http://www.semanticweb.org/alex/ontologies/2024/4/Flight_Satisfaction_Surveys/HybridInternationalAirline">
        <rdfs:subClassOf rdf:resource="http://www.semanticweb.org/alex/ontologies/2024/4/Flight_Satisfaction_Surveys/InternationalAirline"/>
        <rdfs:comment>Represents an international airline company that combines elements of both full-service and low-cost carriers, providing a mix of amenities and services.</rdfs:comment>
        <rdfs:label>Hybrid International Airline</rdfs:label>
    </owl:Class>
    


    <!-- http://www.semanticweb.org/alex/ontologies/2024/4/Flight_Satisfaction_Surveys/ImmigrationProcessSurvey -->


    <owl:Class rdf:about="http://www.semanticweb.org/alex/ontologies/2024/4/Flight_Satisfaction_Surveys/ImmigrationProcessSurvey">
        <rdfs:subClassOf rdf:resource="http://www.semanticweb.org/alex/ontologies/2024/4/Flight_Satisfaction_Surveys/PostFlightSurvey"/>
        <rdfs:comment>Represents a survey used to gather feedback from passengers about their experience with immigration procedures and processes upon arrival at an international destination.</rdfs:comment>
        <rdfs:label>Immigration Process Survey</rdfs:label>
    </owl:Class>
    


    <!-- http://www.semanticweb.org/alex/ontologies/2024/4/Flight_Satisfaction_Surveys/InternationalAirline -->


    <owl:Class rdf:about="http://www.semanticweb.org/alex/ontologies/2024/4/Flight_Satisfaction_Surveys/InternationalAirline">
        <rdfs:subClassOf rdf:resource="http://www.semanticweb.org/alex/ontologies/2024/4/Flight_Satisfaction_Surveys/FlightDetails"/>
        <rdfs:comment>Represents an airline company that operates flights primarily between different countries or regions.</rdfs:comment>
        <rdfs:label>International Airline</rdfs:label>
    </owl:Class>
    


    <!-- http://www.semanticweb.org/alex/ontologies/2024/4/Flight_Satisfaction_Surveys/InternationalFlight -->


    <owl:Class rdf:about="http://www.semanticweb.org/alex/ontologies/2024/4/Flight_Satisfaction_Surveys/InternationalFlight">
        <rdfs:subClassOf rdf:resource="http://www.semanticweb.org/alex/ontologies/2024/4/Flight_Satisfaction_Surveys/Airline"/>
        <rdfs:comment>Represents a flight that operates between different countries or across international boundaries.</rdfs:comment>
        <rdfs:label>International Flight</rdfs:label>
        <rdfs:sameAs>http://dbpedia.org/resource/International_flight</rdfs:sameAs>
    </owl:Class>
    


    <!-- http://www.semanticweb.org/alex/ontologies/2024/4/Flight_Satisfaction_Surveys/InternationalLongHaulFlight -->


    <owl:Class rdf:about="http://www.semanticweb.org/alex/ontologies/2024/4/Flight_Satisfaction_Surveys/InternationalLongHaulFlight">
        <rdfs:subClassOf rdf:resource="http://www.semanticweb.org/alex/ontologies/2024/4/Flight_Satisfaction_Surveys/LongHaulFlight"/>
        <rdfs:comment>Represents a long-haul flight operating between countries or regions, covering extensive distances.</rdfs:comment>
        <rdfs:label>International Long Haul Flight</rdfs:label>
    </owl:Class>
    


    <!-- http://www.semanticweb.org/alex/ontologies/2024/4/Flight_Satisfaction_Surveys/InternationalRegionalAirline -->


    <owl:Class rdf:about="http://www.semanticweb.org/alex/ontologies/2024/4/Flight_Satisfaction_Surveys/InternationalRegionalAirline">
        <rdfs:subClassOf rdf:resource="http://www.semanticweb.org/alex/ontologies/2024/4/Flight_Satisfaction_Surveys/RegionalAirline"/>
        <rdfs:comment>Represents a regional airline providing flight services to international destinations within a specific geographical region.</rdfs:comment>
        <rdfs:label>International Regional Airline</rdfs:label>
    </owl:Class>
    


    <!-- http://www.semanticweb.org/alex/ontologies/2024/4/Flight_Satisfaction_Surveys/LeisureTraveler -->


    <owl:Class rdf:about="http://www.semanticweb.org/alex/ontologies/2024/4/Flight_Satisfaction_Surveys/LeisureTraveler">
        <rdfs:subClassOf rdf:resource="http://www.semanticweb.org/alex/ontologies/2024/4/Flight_Satisfaction_Surveys/Passenger"/>
        <rdfs:comment>Represents a passenger who travels for leisure purposes, such as vacations, holidays, or recreational activities.</rdfs:comment>
        <rdfs:label>Leisure Traveler</rdfs:label>
    </owl:Class>
    


    <!-- http://www.semanticweb.org/alex/ontologies/2024/4/Flight_Satisfaction_Surveys/LongDomesticFlight -->


    <owl:Class rdf:about="http://www.semanticweb.org/alex/ontologies/2024/4/Flight_Satisfaction_Surveys/LongDomesticFlight">
        <rdfs:subClassOf rdf:resource="http://www.semanticweb.org/alex/ontologies/2024/4/Flight_Satisfaction_Surveys/DomesticFlight"/>
        <rdfs:comment>Represents a domestic flight with a relatively long duration, normally covering extensive distances within a country or region.</rdfs:comment>
        <rdfs:label>Long Domestic Flight</rdfs:label>
    </owl:Class>
    


    <!-- http://www.semanticweb.org/alex/ontologies/2024/4/Flight_Satisfaction_Surveys/LongHaulFlight -->


    <owl:Class rdf:about="http://www.semanticweb.org/alex/ontologies/2024/4/Flight_Satisfaction_Surveys/LongHaulFlight">
        <rdfs:subClassOf rdf:resource="http://www.semanticweb.org/alex/ontologies/2024/4/Flight_Satisfaction_Surveys/Airline"/>
        <rdfs:comment>Represents a flight with a relatively long duration, normally more than seven hours and covering extensive distances, often between continents.</rdfs:comment>
        <rdfs:label>Long Haul Flight</rdfs:label>
    </owl:Class>
    


    <!-- http://www.semanticweb.org/alex/ontologies/2024/4/Flight_Satisfaction_Surveys/LongInternationalFlight -->


    <owl:Class rdf:about="http://www.semanticweb.org/alex/ontologies/2024/4/Flight_Satisfaction_Surveys/LongInternationalFlight">
        <rdfs:subClassOf rdf:resource="http://www.semanticweb.org/alex/ontologies/2024/4/Flight_Satisfaction_Surveys/InternationalFlight"/>
        <rdfs:comment>Represents an international flight with a relatively long duration, normally covering extensive distances between countries or regions.</rdfs:comment>
        <rdfs:label>Long International Flight</rdfs:label>
    </owl:Class>
    


    <!-- http://www.semanticweb.org/alex/ontologies/2024/4/Flight_Satisfaction_Surveys/LowCostCarrier -->


    <owl:Class rdf:about="http://www.semanticweb.org/alex/ontologies/2024/4/Flight_Satisfaction_Surveys/LowCostCarrier">
        <rdfs:subClassOf rdf:resource="http://www.semanticweb.org/alex/ontologies/2024/4/Flight_Satisfaction_Surveys/FlightDetails"/>
        <rdfs:comment>Represents an airline company that offers low-cost flight services, normally with fewer amenities and services compared to traditional airlines.</rdfs:comment>
        <rdfs:label>Low Cost Carrier</rdfs:label>
        <rdfs:sameAs>http://dbpedia.org/resource/Low-cost_carrier</rdfs:sameAs>
    </owl:Class>
    


    <!-- http://www.semanticweb.org/alex/ontologies/2024/4/Flight_Satisfaction_Surveys/LoyaltySurvey -->


    <owl:Class rdf:about="http://www.semanticweb.org/alex/ontologies/2024/4/Flight_Satisfaction_Surveys/LoyaltySurvey">
        <rdfs:subClassOf rdf:resource="http://www.semanticweb.org/alex/ontologies/2024/4/Flight_Satisfaction_Surveys/CustomerSurvey"/>
        <rdfs:comment>Represents a survey aimed at assessing the loyalty, retention, and engagement of customers towards a brand, company, or organization.</rdfs:comment>
        <rdfs:label>Loyalty Survey</rdfs:label>
    </owl:Class>
    


    <!-- http://www.semanticweb.org/alex/ontologies/2024/4/Flight_Satisfaction_Surveys/MaintenanceStaffSurvey -->


    <owl:Class rdf:about="http://www.semanticweb.org/alex/ontologies/2024/4/Flight_Satisfaction_Surveys/MaintenanceStaffSurvey">
        <rdfs:subClassOf rdf:resource="http://www.semanticweb.org/alex/ontologies/2024/4/Flight_Satisfaction_Surveys/EmployeeSurvey"/>
        <rdfs:comment>Represents a survey used to gather feedback from maintenance staff employees, such as aircraft technicians and engineers, about their job satisfaction and work conditions.</rdfs:comment>
        <rdfs:label>Maintenance Staff Survey</rdfs:label>
    </owl:Class>
    


    <!-- http://www.semanticweb.org/alex/ontologies/2024/4/Flight_Satisfaction_Surveys/Passenger -->


    <owl:Class rdf:about="http://www.semanticweb.org/alex/ontologies/2024/4/Flight_Satisfaction_Surveys/Passenger">
        <rdfs:comment>It represents a traveler taking a flight operated by an airline.</rdfs:comment>
        <rdfs:label>Passenger</rdfs:label>
    </owl:Class>
    


    <!-- http://www.semanticweb.org/alex/ontologies/2024/4/Flight_Satisfaction_Surveys/PlusEconomyClassPassenger -->


    <owl:Class rdf:about="http://www.semanticweb.org/alex/ontologies/2024/4/Flight_Satisfaction_Surveys/PlusEconomyClassPassenger">
        <rdfs:subClassOf rdf:resource="http://www.semanticweb.org/alex/ontologies/2024/4/Flight_Satisfaction_Surveys/EconomyClassPassenger"/>
        <rdfs:comment>Represents a passenger traveling in the plus or upgraded economy class cabin of an aircraft, offering additional amenities and services compared to standard economy class.</rdfs:comment>
        <rdfs:label>Plus Economy Class Passenger</rdfs:label>
    </owl:Class>
    


    <!-- http://www.semanticweb.org/alex/ontologies/2024/4/Flight_Satisfaction_Surveys/PostFlightSurvey -->


    <owl:Class rdf:about="http://www.semanticweb.org/alex/ontologies/2024/4/Flight_Satisfaction_Surveys/PostFlightSurvey">
        <rdfs:subClassOf rdf:resource="http://www.semanticweb.org/alex/ontologies/2024/4/Flight_Satisfaction_Surveys/FlightSurvey"/>
        <rdfs:comment>Represents a more specific survey used to gather feedback from passengers about their experience after completing a flight, including arrival procedures and baggage claim.</rdfs:comment>
        <rdfs:label>Post Flight Survey</rdfs:label>
    </owl:Class>
    


    <!-- http://www.semanticweb.org/alex/ontologies/2024/4/Flight_Satisfaction_Surveys/PremiumBusinessClassPassenger -->


    <owl:Class rdf:about="http://www.semanticweb.org/alex/ontologies/2024/4/Flight_Satisfaction_Surveys/PremiumBusinessClassPassenger">
        <rdfs:subClassOf rdf:resource="http://www.semanticweb.org/alex/ontologies/2024/4/Flight_Satisfaction_Surveys/BusinessClassPassenger"/>
        <rdfs:comment>Represents a passenger traveling in the premium or upgraded business class cabin of an aircraft, offering enhanced amenities, services, and comfort.</rdfs:comment>
        <rdfs:label>Premium Business Class Passenger</rdfs:label>
    </owl:Class>
    


    <!-- http://www.semanticweb.org/alex/ontologies/2024/4/Flight_Satisfaction_Surveys/RegionalAirline -->


    <owl:Class rdf:about="http://www.semanticweb.org/alex/ontologies/2024/4/Flight_Satisfaction_Surveys/RegionalAirline">
        <rdfs:subClassOf rdf:resource="http://www.semanticweb.org/alex/ontologies/2024/4/Flight_Satisfaction_Surveys/FlightDetails"/>
        <rdfs:comment>Represents an airline company that operates flights within a specific geographical region, often connecting smaller cities and towns.</rdfs:comment>
        <rdfs:label>Regional Airline</rdfs:label>
    </owl:Class>
    


    <!-- http://www.semanticweb.org/alex/ontologies/2024/4/Flight_Satisfaction_Surveys/RegionalLowCostCarrier -->


    <owl:Class rdf:about="http://www.semanticweb.org/alex/ontologies/2024/4/Flight_Satisfaction_Surveys/RegionalLowCostCarrier">
        <rdfs:subClassOf rdf:resource="http://www.semanticweb.org/alex/ontologies/2024/4/Flight_Satisfaction_Surveys/LowCostCarrier"/>
        <rdfs:comment>Represents a low-cost carrier focusing on providing affordable flight services within a specific region or country.</rdfs:comment>
        <rdfs:label>Regional Low Cost Carrier</rdfs:label>
    </owl:Class>
    


    <!-- http://www.semanticweb.org/alex/ontologies/2024/4/Flight_Satisfaction_Surveys/SatisfactionSurvey -->


    <owl:Class rdf:about="http://www.semanticweb.org/alex/ontologies/2024/4/Flight_Satisfaction_Surveys/SatisfactionSurvey">
        <rdfs:subClassOf rdf:resource="http://www.semanticweb.org/alex/ontologies/2024/4/Flight_Satisfaction_Surveys/CustomerSurvey"/>
        <rdfs:comment>Represents a survey focused on measuring the level of satisfaction or contentment of customers about the flight service.</rdfs:comment>
        <rdfs:label>Satisfaction Survey</rdfs:label>
    </owl:Class>
    


    <!-- http://www.semanticweb.org/alex/ontologies/2024/4/Flight_Satisfaction_Surveys/ShortDomesticFlight -->


    <owl:Class rdf:about="http://www.semanticweb.org/alex/ontologies/2024/4/Flight_Satisfaction_Surveys/ShortDomesticFlight">
        <rdfs:subClassOf rdf:resource="http://www.semanticweb.org/alex/ontologies/2024/4/Flight_Satisfaction_Surveys/DomesticFlight"/>
        <rdfs:comment>Represents a domestic flight with a relatively short duration, normally covering distances within a certain range.</rdfs:comment>
        <rdfs:label>Short Domestic Flight</rdfs:label>
    </owl:Class>
    


    <!-- http://www.semanticweb.org/alex/ontologies/2024/4/Flight_Satisfaction_Surveys/ShortInternationalFlight -->


    <owl:Class rdf:about="http://www.semanticweb.org/alex/ontologies/2024/4/Flight_Satisfaction_Surveys/ShortInternationalFlight">
        <rdfs:subClassOf rdf:resource="http://www.semanticweb.org/alex/ontologies/2024/4/Flight_Satisfaction_Surveys/InternationalFlight"/>
        <rdfs:comment>Represents an international flight with a relatively short duration, normally covering distances within a certain range between countries or regions.</rdfs:comment>
        <rdfs:label>Short International Flight</rdfs:label>
    </owl:Class>
    


    <!-- http://www.semanticweb.org/alex/ontologies/2024/4/Flight_Satisfaction_Surveys/SoloLeisureTraveler -->


    <owl:Class rdf:about="http://www.semanticweb.org/alex/ontologies/2024/4/Flight_Satisfaction_Surveys/SoloLeisureTraveler">
        <rdfs:subClassOf rdf:resource="http://www.semanticweb.org/alex/ontologies/2024/4/Flight_Satisfaction_Surveys/LeisureTraveler"/>
        <rdfs:comment>Represents a leisure traveler who travels alone for personal enjoyment, relaxation, or exploration, seeking travel experiences tailored to individual preferences.</rdfs:comment>
        <rdfs:label>Solo Leisure Traveler</rdfs:label>
    </owl:Class>
    


    <!-- http://www.semanticweb.org/alex/ontologies/2024/4/Flight_Satisfaction_Surveys/StandardBusinessClassPassenger -->


    <owl:Class rdf:about="http://www.semanticweb.org/alex/ontologies/2024/4/Flight_Satisfaction_Surveys/StandardBusinessClassPassenger">
        <rdfs:subClassOf rdf:resource="http://www.semanticweb.org/alex/ontologies/2024/4/Flight_Satisfaction_Surveys/BusinessClassPassenger"/>
        <rdfs:comment>Represents a passenger traveling in the standard business class cabin of an aircraft, offering typical amenities and services for business-class passengers.</rdfs:comment>
        <rdfs:label>Standard Business Class Passenger</rdfs:label>
    </owl:Class>
    


    <!-- http://www.semanticweb.org/alex/ontologies/2024/4/Flight_Satisfaction_Surveys/StandardFrequentFlyer -->


    <owl:Class rdf:about="http://www.semanticweb.org/alex/ontologies/2024/4/Flight_Satisfaction_Surveys/StandardFrequentFlyer">
        <rdfs:subClassOf rdf:resource="http://www.semanticweb.org/alex/ontologies/2024/4/Flight_Satisfaction_Surveys/FrequentFlyer"/>
        <rdfs:comment>Represents a frequent flyer enrolled in an airline&apos;s loyalty program, earning rewards and benefits based on their travel activity.</rdfs:comment>
        <rdfs:label>Standard Frequent Flyer</rdfs:label>
    </owl:Class>
    


    <!-- http://www.semanticweb.org/alex/ontologies/2024/4/Flight_Satisfaction_Surveys/UltraLowCostCarrier -->


    <owl:Class rdf:about="http://www.semanticweb.org/alex/ontologies/2024/4/Flight_Satisfaction_Surveys/UltraLowCostCarrier">
        <rdfs:subClassOf rdf:resource="http://www.semanticweb.org/alex/ontologies/2024/4/Flight_Satisfaction_Surveys/LowCostCarrier"/>
        <rdfs:comment>Represents an airline company offering extremely budget-friendly flight services with minimal amenities and additional charges.</rdfs:comment>
        <rdfs:label>Ultra Low Cost Carrier</rdfs:label>
    </owl:Class>
    


    <!-- 
    ///////////////////////////////////////////////////////////////////////////////////////
    //
    // Individuals
    //
    ///////////////////////////////////////////////////////////////////////////////////////
     -->


    


    <!-- http://www.semanticweb.org/alex/ontologies/2024/4/Flight_Satisfaction_Surveys/BusinessClassPassengerInstance -->


    <owl:NamedIndividual rdf:about="http://www.semanticweb.org/alex/ontologies/2024/4/Flight_Satisfaction_Surveys/BusinessClassPassengerInstance">
        <rdf:type rdf:resource="http://www.semanticweb.org/alex/ontologies/2024/4/Flight_Satisfaction_Surveys/BusinessClassPassenger"/>
        <rdfs:comment>Instance for &apos;Business Class Passenger&apos;</rdfs:comment>
        <rdfs:label>Business Class Passenger Instance</rdfs:label>
    </owl:NamedIndividual>
    


    <!-- http://www.semanticweb.org/alex/ontologies/2024/4/Flight_Satisfaction_Surveys/CustomerSurveyIntance -->


    <owl:NamedIndividual rdf:about="http://www.semanticweb.org/alex/ontologies/2024/4/Flight_Satisfaction_Surveys/CustomerSurveyIntance">
        <rdf:type rdf:resource="http://www.semanticweb.org/alex/ontologies/2024/4/Flight_Satisfaction_Surveys/CustomerSurvey"/>
        <rdfs:comment>Instance for &apos;Customer Survey&apos;</rdfs:comment>
        <rdfs:label>Customer Survey Instance</rdfs:label>
    </owl:NamedIndividual>
    


    <!-- http://www.semanticweb.org/alex/ontologies/2024/4/Flight_Satisfaction_Surveys/DomesticFlightInstance -->


    <owl:NamedIndividual rdf:about="http://www.semanticweb.org/alex/ontologies/2024/4/Flight_Satisfaction_Surveys/DomesticFlightInstance">
        <rdf:type rdf:resource="http://www.semanticweb.org/alex/ontologies/2024/4/Flight_Satisfaction_Surveys/DomesticFlight"/>
        <rdfs:comment>Instance for &apos;Domestic Flight&apos;</rdfs:comment>
        <rdfs:label>Domestic Flight Instance</rdfs:label>
    </owl:NamedIndividual>
    


    <!-- http://www.semanticweb.org/alex/ontologies/2024/4/Flight_Satisfaction_Surveys/FrequentFlyerInstance -->


    <owl:NamedIndividual rdf:about="http://www.semanticweb.org/alex/ontologies/2024/4/Flight_Satisfaction_Surveys/FrequentFlyerInstance">
        <rdf:type rdf:resource="http://www.semanticweb.org/alex/ontologies/2024/4/Flight_Satisfaction_Surveys/FrequentFlyer"/>
        <rdfs:comment>Instance for &apos;Frequent Flyer&apos;</rdfs:comment>
        <rdfs:label>Frequent Flyer Instance</rdfs:label>
    </owl:NamedIndividual>
    


    <!-- http://www.semanticweb.org/alex/ontologies/2024/4/Flight_Satisfaction_Surveys/InternationalFlightInstance -->


    <owl:NamedIndividual rdf:about="http://www.semanticweb.org/alex/ontologies/2024/4/Flight_Satisfaction_Surveys/InternationalFlightInstance">
        <rdf:type rdf:resource="http://www.semanticweb.org/alex/ontologies/2024/4/Flight_Satisfaction_Surveys/InternationalFlight"/>
        <rdfs:comment>Instance for &apos;International Flight&apos;</rdfs:comment>
        <rdfs:label>International Flight Instance</rdfs:label>
    </owl:NamedIndividual>
    


    <!-- http://www.semanticweb.org/alex/ontologies/2024/4/Flight_Satisfaction_Surveys/LongHaulFlightInstance -->


    <owl:NamedIndividual rdf:about="http://www.semanticweb.org/alex/ontologies/2024/4/Flight_Satisfaction_Surveys/LongHaulFlightInstance">
        <rdf:type rdf:resource="http://www.semanticweb.org/alex/ontologies/2024/4/Flight_Satisfaction_Surveys/LongHaulFlight"/>
        <rdfs:comment>Instance for &apos;Long Haul Flight&apos;</rdfs:comment>
        <rdfs:label>Long Haul Flight Instance</rdfs:label>
    </owl:NamedIndividual>
    


    <!-- 
    ///////////////////////////////////////////////////////////////////////////////////////
    //
    // Rules
    //
    ///////////////////////////////////////////////////////////////////////////////////////
     -->


    <rdf:Description rdf:about="urn:swrl:var#flight">
        <rdf:type rdf:resource="http://www.w3.org/2003/11/swrl#Variable"/>
    </rdf:Description>
    <rdf:Description rdf:about="urn:swrl:var#duration">
        <rdf:type rdf:resource="http://www.w3.org/2003/11/swrl#Variable"/>
    </rdf:Description>
    <rdf:Description rdf:about="urn:swrl:var#p">
        <rdf:type rdf:resource="http://www.w3.org/2003/11/swrl#Variable"/>
    </rdf:Description>
    <rdf:Description rdf:about="urn:swrl:var#passenger">
        <rdf:type rdf:resource="http://www.w3.org/2003/11/swrl#Variable"/>
    </rdf:Description>
    <rdf:Description rdf:about="urn:swrl:var#frequency">
        <rdf:type rdf:resource="http://www.w3.org/2003/11/swrl#Variable"/>
    </rdf:Description>
    <rdf:Description>
        <rdf:type rdf:resource="http://www.w3.org/2003/11/swrl#Imp"/>
        <swrl:body>
            <rdf:Description>
                <rdf:type rdf:resource="http://www.w3.org/2003/11/swrl#AtomList"/>
                <rdf:first>
                    <rdf:Description>
                        <rdf:type rdf:resource="http://www.w3.org/2003/11/swrl#ClassAtom"/>
                        <swrl:classPredicate rdf:resource="http://www.semanticweb.org/alex/ontologies/2024/4/Flight_Satisfaction_Surveys/FlightDetails"/>
                        <swrl:argument1 rdf:resource="urn:swrl:var#flight"/>
                    </rdf:Description>
                </rdf:first>
                <rdf:rest>
                    <rdf:Description>
                        <rdf:type rdf:resource="http://www.w3.org/2003/11/swrl#AtomList"/>
                        <rdf:first>
                            <rdf:Description>
                                <rdf:type rdf:resource="http://www.w3.org/2003/11/swrl#IndividualPropertyAtom"/>
                                <swrl:propertyPredicate rdf:resource="http://www.semanticweb.org/alex/ontologies/2024/4/Flight_Satisfaction_Surveys/hasFlightDuration"/>
                                <swrl:argument1 rdf:resource="urn:swrl:var#flight"/>
                                <swrl:argument2 rdf:resource="urn:swrl:var#duration"/>
                            </rdf:Description>
                        </rdf:first>
                        <rdf:rest>
                            <rdf:Description>
                                <rdf:type rdf:resource="http://www.w3.org/2003/11/swrl#AtomList"/>
                                <rdf:first>
                                    <rdf:Description>
                                        <rdf:type rdf:resource="http://www.w3.org/2003/11/swrl#BuiltinAtom"/>
                                        <swrl:builtin rdf:resource="http://www.w3.org/2003/11/swrlb#greaterThanOrEqual"/>
                                        <swrl:arguments>
                                            <rdf:Description>
                                                <rdf:type rdf:resource="http://www.w3.org/1999/02/22-rdf-syntax-ns#List"/>
                                                <rdf:first rdf:resource="urn:swrl:var#duration"/>
                                                <rdf:rest>
                                                    <rdf:Description>
                                                        <rdf:type rdf:resource="http://www.w3.org/1999/02/22-rdf-syntax-ns#List"/>
                                                        <rdf:first rdf:datatype="http://www.w3.org/2001/XMLSchema#integer">7</rdf:first>
                                                        <rdf:rest rdf:resource="http://www.w3.org/1999/02/22-rdf-syntax-ns#nil"/>
                                                    </rdf:Description>
                                                </rdf:rest>
                                            </rdf:Description>
                                        </swrl:arguments>
                                    </rdf:Description>
                                </rdf:first>
                                <rdf:rest rdf:resource="http://www.w3.org/1999/02/22-rdf-syntax-ns#nil"/>
                            </rdf:Description>
                        </rdf:rest>
                    </rdf:Description>
                </rdf:rest>
            </rdf:Description>
        </swrl:body>
        <swrl:head>
            <rdf:Description>
                <rdf:type rdf:resource="http://www.w3.org/2003/11/swrl#AtomList"/>
                <rdf:first>
                    <rdf:Description>
                        <rdf:type rdf:resource="http://www.w3.org/2003/11/swrl#ClassAtom"/>
                        <swrl:classPredicate rdf:resource="http://www.semanticweb.org/alex/ontologies/2024/4/Flight_Satisfaction_Surveys/LongHaulFlight"/>
                        <swrl:argument1 rdf:resource="urn:swrl:var#flight"/>
                    </rdf:Description>
                </rdf:first>
                <rdf:rest rdf:resource="http://www.w3.org/1999/02/22-rdf-syntax-ns#nil"/>
            </rdf:Description>
        </swrl:head>
    </rdf:Description>
    <rdf:Description>
        <rdf:type rdf:resource="http://www.w3.org/2003/11/swrl#Imp"/>
        <swrl:body>
            <rdf:Description>
                <rdf:type rdf:resource="http://www.w3.org/2003/11/swrl#AtomList"/>
                <rdf:first>
                    <rdf:Description>
                        <rdf:type rdf:resource="http://www.w3.org/2003/11/swrl#ClassAtom"/>
                        <swrl:classPredicate rdf:resource="http://www.semanticweb.org/alex/ontologies/2024/4/Flight_Satisfaction_Surveys/Passenger"/>
                        <swrl:argument1 rdf:resource="urn:swrl:var#p"/>
                    </rdf:Description>
                </rdf:first>
                <rdf:rest>
                    <rdf:Description>
                        <rdf:type rdf:resource="http://www.w3.org/2003/11/swrl#AtomList"/>
                        <rdf:first>
                            <rdf:Description>
                                <rdf:type rdf:resource="http://www.w3.org/2003/11/swrl#ClassAtom"/>
                                <swrl:classPredicate rdf:resource="http://www.semanticweb.org/alex/ontologies/2024/4/Flight_Satisfaction_Surveys/FrequentFlyer"/>
                                <swrl:argument1 rdf:resource="urn:swrl:var#p"/>
                            </rdf:Description>
                        </rdf:first>
                        <rdf:rest rdf:resource="http://www.w3.org/1999/02/22-rdf-syntax-ns#nil"/>
                    </rdf:Description>
                </rdf:rest>
            </rdf:Description>
        </swrl:body>
        <swrl:head>
            <rdf:Description>
                <rdf:type rdf:resource="http://www.w3.org/2003/11/swrl#AtomList"/>
                <rdf:first>
                    <rdf:Description>
                        <rdf:type rdf:resource="http://www.w3.org/2003/11/swrl#ClassAtom"/>
                        <swrl:classPredicate rdf:resource="http://www.semanticweb.org/alex/ontologies/2024/4/Flight_Satisfaction_Surveys/FrequentFlyer"/>
                        <swrl:argument1 rdf:resource="urn:swrl:var#p"/>
                    </rdf:Description>
                </rdf:first>
                <rdf:rest rdf:resource="http://www.w3.org/1999/02/22-rdf-syntax-ns#nil"/>
            </rdf:Description>
        </swrl:head>
    </rdf:Description>
    <rdf:Description>
        <rdf:type rdf:resource="http://www.w3.org/2003/11/swrl#Imp"/>
        <swrl:body>
            <rdf:Description>
                <rdf:type rdf:resource="http://www.w3.org/2003/11/swrl#AtomList"/>
                <rdf:first>
                    <rdf:Description>
                        <rdf:type rdf:resource="http://www.w3.org/2003/11/swrl#ClassAtom"/>
                        <swrl:classPredicate rdf:resource="http://www.semanticweb.org/alex/ontologies/2024/4/Flight_Satisfaction_Surveys/Passenger"/>
                        <swrl:argument1 rdf:resource="urn:swrl:var#passenger"/>
                    </rdf:Description>
                </rdf:first>
                <rdf:rest>
                    <rdf:Description>
                        <rdf:type rdf:resource="http://www.w3.org/2003/11/swrl#AtomList"/>
                        <rdf:first>
                            <rdf:Description>
                                <rdf:type rdf:resource="http://www.w3.org/2003/11/swrl#ClassAtom"/>
                                <swrl:classPredicate rdf:resource="http://www.semanticweb.org/alex/ontologies/2024/4/Flight_Satisfaction_Surveys/FrequentFlyer"/>
                                <swrl:argument1 rdf:resource="urn:swrl:var#passenger"/>
                            </rdf:Description>
                        </rdf:first>
                        <rdf:rest>
                            <rdf:Description>
                                <rdf:type rdf:resource="http://www.w3.org/2003/11/swrl#AtomList"/>
                                <rdf:first>
                                    <rdf:Description>
                                        <rdf:type rdf:resource="http://www.w3.org/2003/11/swrl#IndividualPropertyAtom"/>
                                        <swrl:propertyPredicate rdf:resource="http://www.semanticweb.org/alex/ontologies/2024/4/Flight_Satisfaction_Surveys/hasFlightFrequency"/>
                                        <swrl:argument1 rdf:resource="urn:swrl:var#passenger"/>
                                        <swrl:argument2 rdf:resource="urn:swrl:var#frequency"/>
                                    </rdf:Description>
                                </rdf:first>
                                <rdf:rest>
                                    <rdf:Description>
                                        <rdf:type rdf:resource="http://www.w3.org/2003/11/swrl#AtomList"/>
                                        <rdf:first>
                                            <rdf:Description>
                                                <rdf:type rdf:resource="http://www.w3.org/2003/11/swrl#BuiltinAtom"/>
                                                <swrl:builtin rdf:resource="http://www.w3.org/2003/11/swrlb#greaterThanOrEqual"/>
                                                <swrl:arguments>
                                                    <rdf:Description>
                                                        <rdf:type rdf:resource="http://www.w3.org/1999/02/22-rdf-syntax-ns#List"/>
                                                        <rdf:first rdf:resource="urn:swrl:var#frequency"/>
                                                        <rdf:rest>
                                                            <rdf:Description>
                                                                <rdf:type rdf:resource="http://www.w3.org/1999/02/22-rdf-syntax-ns#List"/>
                                                                <rdf:first rdf:datatype="http://www.w3.org/2001/XMLSchema#integer">100</rdf:first>
                                                                <rdf:rest rdf:resource="http://www.w3.org/1999/02/22-rdf-syntax-ns#nil"/>
                                                            </rdf:Description>
                                                        </rdf:rest>
                                                    </rdf:Description>
                                                </swrl:arguments>
                                            </rdf:Description>
                                        </rdf:first>
                                        <rdf:rest rdf:resource="http://www.w3.org/1999/02/22-rdf-syntax-ns#nil"/>
                                    </rdf:Description>
                                </rdf:rest>
                            </rdf:Description>
                        </rdf:rest>
                    </rdf:Description>
                </rdf:rest>
            </rdf:Description>
        </swrl:body>
        <swrl:head>
            <rdf:Description>
                <rdf:type rdf:resource="http://www.w3.org/2003/11/swrl#AtomList"/>
                <rdf:first>
                    <rdf:Description>
                        <rdf:type rdf:resource="http://www.w3.org/2003/11/swrl#ClassAtom"/>
                        <swrl:classPredicate rdf:resource="http://www.semanticweb.org/alex/ontologies/2024/4/Flight_Satisfaction_Surveys/BusinessClassPassenger"/>
                        <swrl:argument1 rdf:resource="urn:swrl:var#passenger"/>
                    </rdf:Description>
                </rdf:first>
                <rdf:rest rdf:resource="http://www.w3.org/1999/02/22-rdf-syntax-ns#nil"/>
            </rdf:Description>
        </swrl:head>
    </rdf:Description>
</rdf:RDF>



<!-- Generated by the OWL API (version 5.1.18) https://github.com/owlcs/owlapi/ -->


